\begin{problem}{2.12}
  Solve the equation
  \begin{align*}
    u_{tt} + u_{xxxx} = 0, \qquad -\infty < x < \infty, \quad t > 0 \\
    u(x, 0) = f(x),\quad u_t(x, 0) = 0 \qquad \text{for $-\infty < x < \infty$}.
  \end{align*}
\end{problem}

\begin{proof}
  Using \eqref{partialy} and \eqref{partialx}, we begin by applying the Fourier transform to the first differential equation yielding
  \begin{align*}
    \fourier{u_{tt} + u_{xxxx}} = \der{t}{2}\left[U(k, t)\right] + k^4 U(k, t) = 0 = \fourier{0}.
  \end{align*}
  This is a second-order linear homogeneous differential equation, the solution to which we readily see is given by
  \begin{align}\label{ode_solution}
    U(k, t) = c_1 \cos(k^2 t) + c_2 \sin(k^2 t).
  \end{align}

  Applying the Fourier transform to the last two equations yields
  \begin{align*}
    \fourier{u(x, 0)} = U(k, 0) = F(k) = \fourier{f(x)}
  \end{align*}
  and
  \begin{align*}
    \fourier{u_t(x, 0)} = \fourier{\left[\frac{\partial u}{\partial t}\right]_{t=0}} &= \left.\der{t}{}\left[U(k, t)\right]\right\rvert_{t=0} = 0 = \fourier{0}.
  \end{align*}

  Using the form \eqref{ode_solution} of the solution we see from the second equation that
  \begin{align*}
    U(k, 0) = c_1 = F(k).
  \end{align*}
  Similarly, we also see from the last equation that
  \begin{align*}
    \der{t}{}\left[U(k, t)\right] = -c_1 k^2 \sin(k^2 t) + c_2 k^2 \cos(k^2 t)
  \end{align*}
  which implies that
  \begin{align*}
    \left.\der{t}{}\left[U(k, t)\right]\right\rvert_{t=0} = c_2 k^2 = 0.
  \end{align*}
  Since this equation must hold for all $k$, this implies that $c_2 = 0$.
  Thus, the solution \eqref{ode_solution} becomes
  \begin{align*}
    U(k,t) = F(k)\cos(k^2t).
  \end{align*}

  From the Convolution Theorem, we see that
  \begin{align*}
    u(x,t) = \fourierinv{F(k)\cos(k^2 t)} &= (f \ast g)(x) \\
    &= \frac{1}{\sqrt{2\pi}} \int_{-\infty}^{\infty}f(x-\xi)g(\xi)d\xi
  \end{align*}
  where $g(x) = \fourierinv{\cos(k^2 t}$.

  Note that it can be shown that
  \begin{align*}
    \frac{1}{\sqrt{2\pi}}\int_{-\infty}^{\infty} e^{ik(x \pm kt)}dk = \frac{1}{2}\left(\frac{(1\pm i)e^{\mp i x^2 / 4t}}{\sqrt{t}}\right).
  \end{align*}
  Thus, using the definition of the complex exponential, we have that
  \begin{align*}
    g(x) &= \fourierinv{\cos(k^2 t)} \\
    &= \frac{1}{2\sqrt{2\pi}}\int_{-\infty}^\infty e^{ik(x + kt)} + e^{ik(x - kt)}dk \\
    &= \frac{1}{4\sqrt{t}}\left[(1+i)e^{-ix^2/4t} + (1-i)e^{ix^2/4t}\right] \\
    &= \frac{1}{2\sqrt{t}}\left[\frac{e^{ix^2/4t} + e^{-ix^2/4t}}{2} + \frac{e^{ix^2/4t} - e^{-ix^2/4t}}{2i}\right] \\
    &= \frac{\cos\left(\frac{x^2}{4t}\right) + \sin\left(\frac{x^2}{4t}\right)}{2\sqrt{t}}.
  \end{align*}
  Therefore, the solution to the original differential equation is given by
  \begin{align*}
    u(x,t)
    &= \frac{1}{\sqrt{2\pi}} \int_{-\infty}^{\infty}f(x-\xi)g(\xi)d\xi \\
    &= \frac{1}{2\sqrt{2\pi t}} \int_{-\infty}^{\infty} f(x-\xi)\left(\cos\left(\frac{\xi^2}{4t}\right) + \sin\left(\frac{\xi^2}{4t}\right)\right) d\xi.
  \end{align*}

\end{proof}
\newpage
