\begin{problem}{2.15}
  Find the Fourier sine transform of the following functions:
  \begin{enumerate}
    \item[a.] $x e^{-a x}$, $a > 0$.
    \item [b.] $\displaystyle \frac{e^{-ax}}{x}$, $a > 0$.
  \end{enumerate}
\end{problem}

\begin{proof}
  Recall that the definition of the Fourier sine transform of a function $f(x)$
  is given by
  \begin{align*}
    \fouriersin{f(x)} = \sqrt{\frac{2}{\pi}} \int_0^\infty \sin kx f(x) dx.
  \end{align*}
  \begin{enumerate}
    \item[a.] From the definition of the Fourier sine transform we have that
      \begin{align*}
        \fouriersin{xe^{-ax}} = \sqrt{\frac{2}{\pi}} \int_0^\infty x e^{-ax}\sin kx  dx.
      \end{align*}

      Using the definition of the complex exponential, we see that
      \begin{align*}
        \fouriersin{xe^{-ax}}
        &= \sqrt{\frac{2}{\pi}} \int_0^\infty x e^{-ax}\left[\frac{e^{ikx} - e^{-ikx}}{2i}\right]  dx \\
        &= -\frac{i}{\sqrt{2\pi}} \int_0^\infty x \left[e^{-(a-ik)x} - e^{-(a+ik)x}\right]  dx.
      \end{align*}

      Now, for $w = a \pm ik$ with $a > 0$, we see using integration by parts with $u = x$ and $dv =e^{-wx}dx$ that
      \begin{align*}
        \int_{0}^\infty x e^{-wx}dx = \left.-\frac{xe^{-wx}}{w}\right\rvert_{0}^\infty + \frac{1}{w} \int_0^\infty e^{-wx} dx.
      \end{align*}

      Note that
      \begin{align*}
        \lim_{x\to\infty} \left| e^{-wx} \right| = \lim_{x\to\infty} \left|e^{-(a\pm ik)x}\right| = \lim_{x\to\infty} \left|e^{-ax}\right|  \left|e^{\mp ikx}\right| \leq \lim_{x\to\infty} \left|e^{-ax}\right|  = 0.
      \end{align*}

      This implies that $\lim_{x\to\infty} e^{-wx} = 0$. Thus,
      \begin{align*}
        \int_{0}^\infty x e^{-wx}dx &= \left.-\frac{xe^{-wx}}{w}\right\rvert_{0}^\infty + \frac{1}{w} \int_0^\infty e^{-wx} dx \\
        &=  -\frac{1}{w^2} \left[ \left.e^{-wx}\right\rvert_{0}^{\infty} \right] \\
        &= \frac{1}{w^2}.
      \end{align*}

      Therefore,
      \begin{align*}
        \fouriersin{xe^{-ax}} &= -\frac{i}{\sqrt{2\pi}}\left[\int_0^\infty x e^{-(a-ik)x}dx - \int_0^\infty x e^{-(a+ik)x}dx\right] \\
        &= -\frac{i}{\sqrt{2\pi}}\left[\frac{1}{(a-ik)^2} - \frac{1}{(a+ik)^2}\right] \\
        &= \sqrt{\frac{2}{\pi}}\frac{2 ak}{\left(a^2 + k^2\right)^2}.
      \end{align*}

    \item[b.] From our table of Fourier sine transforms,
      we see for $a>0$ that
      \begin{align*}
        \fouriersin{e^{-ax}} = \sqrt{\frac{2}{\pi}}\int_{0}^\infty e^{-ax}\sin(kx) dx = \sqrt{\frac{2}{\pi}}\left(\frac{k}{k^2 + a^2}\right).
      \end{align*}

      Thus, we must have that both sides are equal after integrating with respect to $a$ from $a$ to $\infty$, i.e.
      \begin{align*}
        \sqrt{\frac{2}{\pi}}\int_{a}^\infty \left[\int_{0}^\infty e^{-ax}\sin(kx) dx \right]da = \sqrt{\frac{2}{\pi}}\int_a^\infty\left(\frac{k}{k^2 + a^2}\right)da.
      \end{align*}
      For the integral on the left, since the integrand is continuous on the domain of integration, we can interchange the order of integration
      and we see that
      \begin{align*}
        \sqrt{\frac{2}{\pi}}\int_{a}^\infty \left[\int_{0}^\infty e^{-ax}\sin(kx) dx \right]da
        &= \sqrt{\frac{2}{\pi}} \int_{0}^\infty \sin(kx) \left[\int_{a}^\infty  e^{-ax}da \right]dx \\
        &= \sqrt{\frac{2}{\pi}} \int_{0}^\infty \frac{e^{-ax}}{x}\sin(kx) dx \\
        &= \fouriersin{\frac{e^{-ax}}{x}}.
      \end{align*}
      Therefore,
      \begin{align*}
        \fouriersin{\frac{e^{-ax}}{x}} = \sqrt{\frac{2}{\pi}}\int_a^\infty\left(\frac{k}{k^2 + a^2}\right)da.
      \end{align*}
      Note, the indefinite integral evaluates to $\displaystyle \tan^{-1}\left(\frac{a}{k}\right)$ and we
      therefore see that
      \begin{align*}
        \fouriersin{\frac{e^{-ax}}{x}} &= \sqrt{\frac{2}{\pi}}\int_a^\infty\left(\frac{k}{k^2 + a^2}\right)da \\
        &= \sqrt{\frac{2}{\pi}} \left(\left. \tan^{-1}\left(\frac{a}{k}\right) \right\rvert_{a}^\infty\right) \\
        &= \sqrt{\frac{2}{\pi}}\left(\frac{\pi}{2} - \tan^{-1}\left(\frac{a}{k}\right) \right)
      \end{align*}


  \end{enumerate}
\end{proof}
\newpage
