\begin{problem}{4.3}
  Find the solutions of the following systems of equations with the initial data:
  \begin{enumerate}
    \item[a.]
      $
      \begin{array}{ll}
        \frac{dx}{dt} = x - 2y, \quad x(0) = 1 \\
        \frac{dy}{dt} = y - 2x, \quad y(0) = 0
      \end{array}
      $

  \end{enumerate}
\end{problem}

\begin{proof}
  \begin{enumerate}
    \item[a.] Applying the Laplace transform to the system yields
      \begin{align*}
        \laplace{\frac{dx}{dt}} = s\bar{x}(s) - x(0) = \bar{x}(s) - 2 \bar{y}(s) = \laplace{x - 2y} \\
        \laplace{\frac{dy}{dt}} = s\bar{y}(s) - y(0) = \bar{y}(s) - 2 \bar{x}(s) = \laplace{y - 2x}.
      \end{align*}

      Using the initial data, the transformed system becomes
      \begin{align*}
        (s-1)\bar{x}(s) + 2 \bar{y}(s) &= 1\\
        2\bar{x}(s) + (s-1) \bar{y}(s) &= 0,
      \end{align*}
      or, equivalently,
      \begin{align*}
        \begin{bmatrix}
          s-1 & 2 \\
          2 & s-1
        \end{bmatrix}
        \begin{bmatrix}
          \bar{x}(s) \\
          \bar{y}(s)
        \end{bmatrix}
        =
        \begin{bmatrix}
          1 \\
          0
        \end{bmatrix}
      \end{align*}

      This implies that the solution to the transformed system of equations is given by
      \begin{align*}
        \begin{bmatrix}
          \bar{x}(s) \\
          \bar{y}(s)
        \end{bmatrix}
        =
        \begin{bmatrix}
          s-1 & 2 \\
          2 & s-1
        \end{bmatrix}
        ^{-1}
        \begin{bmatrix}
          1 \\
          0
        \end{bmatrix}
        =
        \begin{bmatrix}
          \frac{s-1}{(s-3)(s+1)} & -\frac{2}{(s-3)(s+1)} \\
          -\frac{2}{(s-3)(s+1)} & \frac{s-1}{(s-3)(s+1)}
        \end{bmatrix}
        \begin{bmatrix}
          1 \\
          0
        \end{bmatrix}
        =
        \begin{bmatrix}
          \frac{s-1}{(s-3)(s+1)} \\
          -\frac{2}{(s-3)(s+1)}
        \end{bmatrix}
      \end{align*}
      i.e. the solution is given by $\displaystyle \bar{x}(s) = \frac{s-1}{(s-3)(s+1)}$ and $\displaystyle \bar{y}(s) = -\frac{2}{(s-3)(s+1)}$.

      From our table of Laplace Transforms, we know that
      \begin{align*}
        \laplace{e^{at} - e^{bt}} = \frac{a-b}{(s-a)(s-b)}
      \end{align*}
      and
      \begin{align*}
        \laplace{\frac{ae^{at} - be^{bt}}{a-b}} = \frac{s}{(s-a)(s-b)}.
      \end{align*}

      Therefore, the solution to the original system of differential equations is given by
      \begin{align*}
        x(t) = \laplaceinv{\bar{x}(s)} &= \laplaceinv{\frac{s-1}{(s-3)(s+1)}} \\
        &= \laplaceinv{\frac{s}{(s-3)(s+1)}} - \laplaceinv{\frac{1}{(s-3)(s+1)}} \\
        &= \frac{3e^{3t}+e^{-t}}{4} - \frac{e^{3t} - e^{-t}}{r} \\
        &= \frac{e^{3t} + e^{-t}}{2}
      \end{align*}
      and
      \begin{align*}
        y(t) = \laplaceinv{\bar{y}(s)} &= \laplaceinv{-\frac{2}{(s-3)(s+1)}} \\
        &= \frac{e^{-t} - e^{3t}}{2}
      \end{align*}

  \end{enumerate}
\end{proof}
\newpage
