\begin{problem}{7.19}
  Use the joint Hankel and Laplace transform method to solve the initial boundary value problem
  \begin{align*}
    &u_{rr} + \frac{1}{r}u_r - u_{tt} - 2 \varepsilon u_t = a \frac{\delta(r)}{r}\delta(t), \qquad 0 < r < \infty, \quad 0 < t, \\
    &u(r, t) \to 0 \qquad \text{as $r \to \infty$}, \\
    &u(0, t) \qquad \text{is finite for $0 < t$}, \\
    &u(r, 0) = u_t(r, 0) = 0 \qquad \text{for $0 < r < \infty$}.
  \end{align*}
\end{problem}

\begin{proof}
  We begin by applying the 0-th order Hankel transform to the differential equation and its initial and boundary conditions. Doing so yields
  \begin{align*}
    &-k^2\tilde{u}_0(k, t) - \der{t}{2}\left[\tilde{u}_0(k, t)\right] -2\varepsilon \der{t}{}\left[\tilde{u}_0(k, t)\right] = a\delta(t), \qquad 0 < r < \infty, \quad 0 < t,\\
    &\tilde{u}_0(k, t) \to 0 \qquad \text{as $k \to \infty$}, \\
    &\tilde{u}_0(0, t) \qquad \text{is finite for $0 < t$}, \\
    &\tilde{u}_0(k, 0) = \left.\der{t}{}\left[\tilde{u}_0(k, t)\right]\right\rvert_{t=0} = 0 \qquad \text{for $0 < k < \infty$}.
  \end{align*}
  Now, let $\bar{\tilde{u}}_0(k, s) = \laplace{\tilde{u}_0(k, t)}$. Applying the Laplace transform to the resulting equation shows that
  \begin{align*}
    -k^2\bar{\tilde{u}}_0(k, s) - s^2\bar{\tilde{u}}_0(k, s) + s \tilde{u}_0(k, 0) +\left.\der{t}{}\left[\tilde{u}_0(k, t)\right]\right\rvert_{t=0} - 2\varepsilon\left(s\bar{\tilde{u}}_0(k, s) - \tilde{u}_0(k, 0)\right) = a.
  \end{align*}

  In light of the initial data, this equation reduces to
  \begin{align*}
    -k^2\bar{\tilde{u}}_0(k, s) - s^2\bar{\tilde{u}}_0(k, s) - 2\varepsilon s \bar{\tilde{u}}_0(k, s) = a,
  \end{align*}
  or, equivalently,
  \begin{align*}
    \left[s^2 + 2\varepsilon s +k^2\right]\bar{\tilde{u}}_0(k, s) = -a.
  \end{align*}
  Thus, the solution to the Laplace-transformed equation is
  \begin{align*}
    \bar{\tilde{u}}_0(k, s) = -\frac{a}{s^2 + 2\varepsilon s +k^2} = -\frac{a}{\left[s - \left(-\varepsilon -\sqrt{\varepsilon^2 - k^2}\right)\right]\left[s- \left(-\varepsilon +\sqrt{\varepsilon^2 - k^2}\right)\right]}.
  \end{align*}

  Recall that
  \begin{align*}
    \frac{1}{a-b}\laplace{e^{at} - e^{bt}} = \frac{1}{(s-a)(s-b)}.
  \end{align*}
  This implies that
  \begin{align*}
    \tilde{u}_0(k, t) = \laplaceinv{\bar{\tilde{u}}_0(k, s)} &= -a\laplaceinv{\frac{1}{\left[s - \left(-\varepsilon -\sqrt{\varepsilon^2 - k^2}\right)\right]\left[s- \left(-\varepsilon +\sqrt{\varepsilon^2 - k^2}\right)\right]}} \\
    &= \frac{a\left[e^{\left(-\varepsilon -\sqrt{\varepsilon^2 - k^2}\right)t} - e^{\left(-\varepsilon +\sqrt{\varepsilon^2 - k^2}\right)t}\right]}{2\sqrt{\varepsilon^2-k^2}}.
  \end{align*}

  Therefore, the solution to the original differential equation is
  \begin{align*}
    u(r, t) = \hankelinv{0}{\tilde{u}_0(k, t)} = \int_0^\infty k \left\{\frac{a\left[e^{\left(-\varepsilon -\sqrt{\varepsilon^2 - k^2}\right)t} - e^{\left(-\varepsilon +\sqrt{\varepsilon^2 - k^2}\right)t}\right]}{2\sqrt{\varepsilon^2-k^2}} \right\}J_0(k r) dk.
  \end{align*}
\end{proof}
\newpage
