\begin{problem}{5}
  Let $p(z)$ be a polynomial of degree $d > 1$ with Newton function
  $$\displaystyle N_p(z) = z - \frac{p(z)}{p'(z)}.$$
  \begin{enumerate}
    \item If $p(\alpha) = 0$ and $p'(\alpha) \neq 0$, show that $\alpha$ is a fixed point
      of multiplicity two for $N_p$, i.e.\ there is a rational function $k(z) = m(z) / n(z)$ with
      $n(\alpha) \neq 0$ and $N_p(z) - \alpha = (z-\alpha)^2 k(z)$.
    \item If $p(\alpha) = 0$, $p'(\alpha) \neq 0$, and $p''(\alpha) = 0$, show that $\alpha$
      is a fixed point of multiplicity three for $N_p$.
  \end{enumerate}
\end{problem}

\begin{proof}
  \begin{enumerate}
    \item If $N_p(z)$ is the Newton function of the polynomial $p(z)$ of degree $n > 1$, then
      \begin{align}\label{newton}
        N_p(z) - \alpha = z - \alpha - \frac{p(z)}{p'(z)} = \frac{(z-\alpha)p'(z) - p(z)}{p'(z)}.
      \end{align}

      Note that if $p(\alpha) = 0$, then
      \begin{align*}
        p(z) = (z-\alpha)\sum_{k=0}^{n-1}a_k z^k.
      \end{align*}
      This implies that
      \begin{align*}
        p'(z) &= \sum_{k=0}^{n-1}a_k z^k + (z-\alpha)\sum_{k=1}^{n-1}k a_k z^{k-1} \\
        &= \sum_{k=0}^{n-1}a_k z^k + (z-\alpha)m(z),
      \end{align*}
      say. Thus, from \eqref{newton}, we see that
      \begin{align*}
        N_p(z) - \alpha &= \frac{(z-\alpha)p'(z) - p(z)}{p'(z)} \\
        &= \frac{p(z) + (z-\alpha)^2m(z) - p(z)}{p'(z)} \\
        &= \frac{(z-\alpha)^2m(z)}{p'(z)}.
      \end{align*}
      Since $p'(\alpha) \neq 0$, set $n(z) = p'(z)$. Then we have from the above
      equation that
      $$N_p(z) - \alpha = (z-\alpha)^2 \frac{m(z)}{n(z)},$$ or that $\alpha$
      is a fixed point of multiplicity two for $N_p$.

    \item Suppose that $p(\alpha) = 0$ and $p'(\alpha) \neq 0$.
      Then as shown previously,
      \begin{align*}
        p'(z) &= \sum_{k=0}^{n-1}a_k z^k + (z-\alpha)\sum_{k=1}^{n-1}k a_k z^{k-1} \\
        &= \sum_{k=0}^{n-1}a_k z^k + (z-\alpha)m(z),
      \end{align*}
      and
      $$N_p(z) - \alpha = (z-\alpha)^2 \frac{m(z)}{p'(z)}.$$
      Thus, $\alpha$ will be a fixed point of multiplicity three for $N_p(z)$
      if $(z-\alpha)$ is a factor of $m(z) = \sum_{k=1}^{n-1}k a_k z^{k-1}$.

      Suppose that $p''(\alpha) = 0$. Then from previous calculations, we see that
      \begin{align*}
        p''(z) &= \left(\sum_{k=0}^{n-1}a_k z^k + (z-\alpha)\sum_{k=1}^{n-1}k a_k z^{k-1}\right)' \\
        &= \sum_{k=1}^{n-1}k a_k z^{k-1} + \sum_{k=1}^{n-1}k a_k z^{k-1} + (z-\alpha)\sum_{k=2}^{n-1}k (k-1) a_k z^{k-2} \\
        &= 2m(z) + (z-\alpha)m'(z).
      \end{align*}
      Now, if $p''(\alpha) = 0$, this implies that $2m(\alpha) = 0$ or that $m(\alpha) = 0$.
      Thus, $\alpha$ is a root of $m(z)$ which implies that $(z-\alpha)$ is a factor of $m(z)$.
      Therefore, $\alpha$ is a fixed point of multiplicity three for $N_p(z)$.
  \end{enumerate}
\end{proof}
\newpage
