\begin{problem}{5}
  Show that
  \begin{align*}
    \int_0^\infty e^{-ax} \left(\frac{\cos p x - \cos q x}{x}\right) dx = \frac{1}{2} \log \frac{q^2 + a^2}{p^2 + a^2}
  \end{align*}
\end{problem}

\begin{proof}
  Recall that the Laplace transform of a function $f(t)$ is defined as
  \begin{align*}
    \bar{f}(s) = \laplace{f(t)}_s = \int_0^\infty f(t) e^{-st} dt
  \end{align*}
  where we explicitly note the transformation variable $s$.
  Thus, we see that the integral above becomes
  \begin{align}
    \label{5:int}
    \int_0^\infty e^{-ax} \left(\frac{\cos p x - \cos q x}{x}\right) dx &= \int_0^\infty e^{-ax} \left(\frac{\cos p x}{x}\right)dx - \int_0^\infty e^{-ax} \left(\frac{\cos q x}{x}\right) dx \notag \\
    &= \laplace{\frac{\cos p x}{x}}_a - \laplace{\frac{\cos q x}{x}}_a.
  \end{align}

  From a previous theorem, if $\laplace{f(t)} = \bar{f}(s)$, then we have that
  \begin{align*}
    \laplace{\frac{f(t)}{t}} = \int_s^\infty \bar{f}(z) dz.
  \end{align*}
  Thus, we see that \eqref{5:int} becomes
  \begin{align*}
    \int_0^\infty e^{-ax} \left(\frac{\cos p x - \cos q x}{x}\right) dx
    &= \laplace{\frac{\cos p x}{x}}_a - \laplace{\frac{\cos q x}{x}}_a \\
    &= \int_a^\infty \laplace{\cos px}_z dz - \int_a^\infty \laplace{\cos qx}_z dz
  \end{align*}
  From the table of Laplace transforms, we have that
  \begin{align*}
    \laplace{\cos b x}_z = \frac{z}{b^2 + z^2}.
  \end{align*}

  Thus, we have that
  \begin{align*}
    \int_0^\infty e^{-ax} \left(\frac{\cos p x - \cos q x}{x}\right) dx
    &= \int_a^\infty \laplace{\cos px}_z dz - \int_a^\infty \laplace{\cos qx}_z dz\\
    &= \int_a^\infty \frac{z}{p^2 + z^2} dz - \int_a^\infty \frac{z}{q^2 + z^2} dz
  \end{align*}

  Using a $u$-substitution to solve the resulting integrals, we have that
  \begin{align*}
    \int_0^\infty e^{-ax} \left(\frac{\cos p x - \cos q x}{x}\right) dx
    &= \int_a^\infty \frac{z}{p^2 + z^2} dz - \int_a^\infty \frac{z}{q^2 + z^2} dz\\
    &= \left.\frac{1}{2}\log p^2 + z^2 \right\rvert_{a}^\infty - \left.\frac{1}{2}\log p^2 + z^2 \right\rvert_{a}^\infty .
  \end{align*}
  Using the properties of logarithms, we therefore see that
  \begin{align*}
    \int_0^\infty e^{-ax} \left(\frac{\cos p x - \cos q x}{x}\right) dx
    &= \left.\frac{1}{2}\log p^2 + z^2 \right\rvert_{a}^\infty - \left.\frac{1}{2}\log p^2 + z^2 \right\rvert_{a}^\infty  \\
    &= \frac{1}{2} \left[\left.\log \frac{p^2 + z^2}{q^2 + z^2}\right\rvert_{z=\infty} - \left.\log \frac{p^2 + z^2}{q^2 + z^2}\right\rvert_{z=a} \right] \\
    &= -\frac{1}{2} \log \frac{p^2 + a^2}{q^2 + a^2} \\
    &= \frac{1}{2} \log \frac{q^2 + a^2}{p^2 + a^2}.
  \end{align*}

\end{proof}
\newpage
