\begin{problem}{2}
  Find the solution of the wave equation by the Hankel transform
  \begin{align*}
    &u_{tt} = c^2\left(u_{rr} + \frac{1}{r}u_r + u_{zz}\right), \qquad 0 < r < \infty, \quad 0 < t, \quad 0 < z\\
    &u_z\rvert_{z=0} = g(r,t)
  \end{align*}
  where $c$ is a constant and $g(r,t)$ is given.
\end{problem}

\begin{proof}
  Suppose that $u(r, z, t) = \phi(r, z) e^{i\omega t}$ and $g(r, t) = f(r) e^{i \omega t}$. Then the wave equation
  becomes
  \begin{align*}
    &c^2 e^{i \omega t} \left(\frac{\partial^2}{\partial r^2}\left[\phi(r, z)\right] + \frac{1}{r}\frac{\partial}{\partial r}\left[\phi(r, z)\right] + \frac{\partial^2}{\partial z^2}\left[\phi(r, z)\right]\right) + \omega^2 e^{i \omega t} \phi(r, z) = 0 \\
    &e^{i\omega t}\left(\left.\frac{\partial}{\partial z}\left[\phi(r,z)\right]\right\rvert_{z=0}- f(r)\right) = 0
  \end{align*}
  for $0 < r < \infty$, $0 < t$, and  $0 < z$.

  Suppose that $\hankel{0}{\phi(r,z)} = \tilde{\phi}_0(\kappa, z)$ and $\hankel{0}{f(r)} = \tilde{f}_0(\kappa)$.
  Then, using \eqref{hankel}, applying the 0-th order Hankel transform with respect to $r$ to the above equation yields
  \begin{align*}
    &e^{i\omega t} \left[c^2 \left(\der{z}{2}\left[\tilde{\phi}_0(\kappa, z)\right] - \kappa^2 \tilde{\phi}_0(\kappa, z) \right) + \omega^2 \tilde{\phi}_0(\kappa, z)\right] = 0, \quad 0 < r < \infty, \quad 0 < t, \quad 0 < z \\
    &e^{i\omega t}\left(\left.\frac{\partial}{\partial z}\left[\tilde{\phi}_0(r,z)\right]\right\rvert_{z=0}- \tilde{f}_0(r)\right) = 0
  \end{align*}
  Since the first equation must hold for all $t>0$, we require that
  \begin{align*}
    c^2 \left(\der{z}{2}\left[\tilde{\phi}_0(\kappa, z)\right] - \kappa^2 \tilde{\phi}_0(\kappa, z) \right) + \omega^2 \tilde{\phi}_0(\kappa, z) = 0.
  \end{align*}
  This is a second-order linear, homogeneous equation, the solution of which is
  \begin{align*}
    \tilde{\phi}_0(\kappa, z) = c_1(\kappa) \exp\left[\frac{\sqrt{(c\kappa)^2-\omega^2}}{c} z\right] + c_2(\kappa) \exp\left[-\frac{\sqrt{(c\kappa)^2-\omega^2}}{c} z\right].
  \end{align*}
  Note that this solution must converge as $z \to \infty$, which implies that $c_2(\kappa) = 0$.
  Then from the above solution we have that
  \begin{align*}
    \frac{\partial}{\partial z}\left[\tilde{\phi}(\kappa, z)\right] = c_1(\kappa)\frac{\sqrt{(c\kappa)^2-\omega^2}}{c} \exp\left[\frac{\sqrt{(c\kappa)^2-\omega^2}}{c} z\right].
  \end{align*}
  Thus, we have that
  \begin{align*}
    \left.\frac{\partial}{\partial z}\left[\tilde{\phi}_0(r,z)\right]\right\rvert_{z=0} = c_1(\kappa)\frac{\sqrt{(c\kappa)^2-\omega^2}}{c}.
  \end{align*}
  Since the transformed boundary condition must hold for all $t > 0$, we must have that
  \begin{align*}
    \left.\frac{\partial}{\partial z}\left[\tilde{\phi}_0(r,z)\right]\right\rvert_{z=0}- \tilde{f}_0(r) = 0
  \end{align*}
  or that
  \begin{align*}
    c_1(\kappa) = \frac{c\tilde{f}_0(\kappa)}{\sqrt{(c\kappa)^2-\omega^2}}.
  \end{align*}
  Thus, the solution to the transformed equation is
  \begin{align*}
    \tilde{\phi}_0(\kappa, z) = \frac{c\tilde{f}_0(\kappa)}{\sqrt{(c\kappa)^2-\omega^2}}\exp\left[\frac{\sqrt{(c\kappa)^2-\omega^2}}{c} z\right].
  \end{align*}

  Therefore, taking the inverse 0-th order Hankel transform, we have that
  \begin{align*}
    \phi(r, z) = \hankelinv{0}{\tilde{\phi}_0(\kappa, z)}
    &= \hankelinv{0}{\frac{c\tilde{f}_0(\kappa)}{\sqrt{(c\kappa)^2-\omega^2}}\exp\left[\frac{\sqrt{(c\kappa)^2-\omega^2}}{c} z\right]} \\
    &= \int_0^\infty \kappa J_0(\kappa r)\left[\frac{c\tilde{f}_0(\kappa)}{\sqrt{(c\kappa)^2-\omega^2}}\exp\left[\frac{\sqrt{(c\kappa)^2-\omega^2}}{c} z\right]\right] d\kappa
  \end{align*}
  and the solution to the original wave equation is
  \begin{align*}
    u(r, z, t) = \phi(r, z)e^{i \omega t} = e^{i\omega t}\int_0^\infty \kappa J_0(\kappa r)\left[\frac{c\tilde{f}_0(\kappa)}{\sqrt{(c\kappa)^2-\omega^2}}\exp\left[\frac{\sqrt{(c\kappa)^2-\omega^2}}{c} z\right]\right] d\kappa.
  \end{align*}
\end{proof}
\newpage
