\begin{problem}{2.7}
  Prove the following results for the convolution:
  \begin{enumerate}
    \item [c.] $\displaystyle \der{x}{}\left[f(x) \ast g(x)\right] = f'(x) \ast g(x) = f(x) \ast g'(x),$
    \item [d.] $\displaystyle \int_{-\infty}^{\infty} (f \ast g)(x) dx = \int_{-\infty}^{\infty} f(u)du \int_{-\infty}^{\infty} g(v)dv.$
  \end{enumerate}
\end{problem}

\begin{proof}
  For two functions functions $f, g \in L^1(\mathbb{R})$, the convolution of $f$ and $g$,
  denoted by $(f \ast g )(x)$, is defined to be
  \begin{align*}
    (f \ast g )(x) = \int_{-\infty}^{\infty} f(x - \xi) g(\xi) d\xi.
  \end{align*}

  \begin{enumerate}
    \item [c.] Using the definition of the convolution of $f$ and $g$, we have that
      \begin{align*}
        \der{x}{}\left[f(x) \ast g(x)\right] &= \der{x}{}\int_{-\infty}^{\infty} f(x - \xi) g(\xi) d\xi \\
        &= \int_{-\infty}^{\infty} \frac{\partial}{\partial x}\left[f(x - \xi) g(\xi)\right] d\xi \\
        &= \int_{-\infty}^{\infty} f'(x - \xi) g(\xi)d\xi \\
        &= f'(x) \ast g(x).
      \end{align*}

      Since the convolution of two functions is commutative, we have using the above that
      \begin{align*}
        \der{x}{}\left[f(x) \ast g(x)\right] &= \der{x}{}\left[g(x) \ast f(x)\right] \\
        &= g'(x) \ast f(x) \\
        &= f(x) \ast g'(x).
      \end{align*}

    \item [d.] From the definition of the convolution of $f$ and $g$, we have that
      \begin{align*}
        \int_{-\infty}^{\infty} (f \ast g)(x) dx &= \int_{-\infty}^{\infty} \left[\int_{-\infty}^{\infty} f(x - \xi) g(\xi) d\xi\right] dx.
      \end{align*}
      Since $f, g \in L^1(\mathbb{R})$, we may interchange the order of integration above. Doing so yields
      \begin{align*}
        \int_{-\infty}^{\infty} (f \ast g)(x) dx
        &= \int_{-\infty}^{\infty} \left[\int_{-\infty}^{\infty} f(x - \xi) g(\xi) d\xi\right] dx\\
        &= \int_{-\infty}^{\infty} g(\xi)\left[\int_{-\infty}^{\infty} f(x - \xi) dx\right] d\xi.
      \end{align*}
      Making the substitution $u= x- \xi$ with $du = dx$, the above becomes
      \begin{align*}
        \int_{-\infty}^{\infty} (f \ast g)(x) dx &= \int_{-\infty}^{\infty} g(\xi)\left[\int_{-\infty}^{\infty} f(x - \xi) dx\right] d\xi\\
        &= \int_{-\infty}^{\infty} g(\xi)\left[\int_{-\infty}^{\infty} f(u) du\right] d\xi \\
        &= \int_{-\infty}^{\infty} g(\xi) d\xi \int_{-\infty}^{\infty} f(u) du.
      \end{align*}
      The variables $u$ and $\xi$ are arbitary; therefore
      \begin{align*}
        \int_{-\infty}^{\infty} (f \ast g)(x) dx = \int_{-\infty}^{\infty} f(u)du \int_{-\infty}^{\infty} g(v)dv
      \end{align*}
      and we are done.
  \end{enumerate}
\end{proof}
\newpage
