\begin{problem}{2.5}
  Prove the following:
  \begin{enumerate}
    \item [c.] If $f(x)$ has a finite discontinuity at a point $x = a$, then
      \begin{align*}
        \fourier{f'(x)} = (ik) F(k) - \frac{1}{\sqrt{2\pi}}\exp(-ika)[f]_a,
      \end{align*}
      where $[f]_a = f(a + 0) - f (a - 0).$

      Generalize this result for $\fourier{f^{(n)}(x)}$.
  \end{enumerate}
\end{problem}

\begin{proof}
  \begin{enumerate}
    \item [c.] Suppose that $f$ has a finite discontinuity at the point $x=a$. From
      the definition of the Fourier transform, we have that
      \begin{align}\label{int}
        \fourier{f'(x)} &= \frac{1}{\sqrt{2\pi}} \int_{-\infty}^{\infty} e^{-ikx} f'(x) dx \notag \\
        &= \frac{1}{\sqrt{2\pi}} \left[\int_{-\infty}^{a} e^{-ikx} f'(x) dx + \int_{a}^{\infty} e^{-ikx} f'(x) dx \right],
      \end{align}
      where we have separated the integral at the finite discontinuity. Since $f(x)$ and $e^{-ikx}$ are both
      continuous with continuous first derivatives on the intervals present in the above two integrals,
      we may apply integration by parts to compute these integrals. Set $u=e^{-ikx}$ and $dv=f'(x)dx$. Then
      $du = -ik e^{-ikx}dx$ and $v = f(x)$ so that
      \begin{align*}
        \int_{-\infty}^{a} e^{-ikx} f'(x) dx &= \left. e^{-ikx}f(x) \right\rvert_{-\infty}^{a^-} + ik \int_{-\infty}^a e^{-ikx}f(x) dx \\
        &= e^{-ika} \lim_{x\to a^{-}}f(x)  + ik \int_{-\infty}^a e^{-ikx}f(x) dx.
      \end{align*}

      Similarly, we also see that
      \begin{align*}
        \int_{a}^{\infty} e^{-ikx} f'(x) dx
        &= \left. e^{-ikx}f(x) \right\rvert_{a^+}^{\infty} + ik \int_{-\infty}^a e^{-ikx}f(x) dx \\
        &= -e^{-ika} \lim_{x\to a^{+}}f(x)  + ik \int_{a}^\infty e^{-ikx}f(x) dx.
      \end{align*}

      Combining, we see therefore from \eqref{int} that
      \begin{align*}
        \fourier{f'(x)} &= \frac{1}{\sqrt{2\pi}} \left[\int_{-\infty}^{a} e^{-ikx} f'(x) dx + \int_{a}^{\infty} e^{-ikx} f'(x) dx \right] \\
        &= \frac{1}{\sqrt{2\pi}} \left[
          e^{-ika} \lim_{x\to a^{-}}f(x)
          -e^{-ika} \lim_{x\to a^{+}}f(x)  + ik \int_{-\infty}^\infty e^{-ikx}f(x) dx
        \right] \\
        &= ik F(k) - \frac{1}{\sqrt{2\pi}}e^{-ika}\left( \lim_{x\to a^+} f(x) - \lim_{x\to a^{-}} f(x)\right) \\
        &= ik F(k) - \frac{1}{\sqrt{2\pi}}e^{-ika} [f]_a
      \end{align*}
      where we have used $\lim_{x\to a^+} f(x) - \lim_{x\to a^{-}} f(x) = f(a+0) - f(a-0) = [f]_a$.

      We now wish to show that, in general,
      \begin{align}\label{ind_four}
        \fourier{f^{(n)}(x)} = (ik)^n F(k) - \frac{1}{\sqrt{2\pi}}e^{-ika}\sum_{j=1}^{n} (ik)^{n-j} [f^{(j-1)}]_a
      \end{align}
      given that $f\in \mathbb{S}$, the set of all good functions.

      We have shown previously that this result holds for $n=1$, so suppose this result
      holds for $n$.
      Then we see that
      \begin{align*}
        \fourier{f^{(n+1)}} &= \frac{1}{\sqrt{2\pi}}\int_{-\infty}^{\infty}e^{-ikx}f^{(n+1)}(x)dx \\
        &= \frac{1}{\sqrt{2\pi}}\left[\int_{-\infty}^{a}e^{-ikx}f^{(n+1)}(x)dx + \int_{-\infty}^{a}e^{-ikx}f^{(n+1)}(x)dx\right].
      \end{align*}
      Proceeding as before, we integrate by parts using the substitution $u = e^{-ikx}$ and $dv = f^{(n+1}(x)dx$ yielding
      \begin{align*}
        \int_{-\infty}^{a}e^{-ikx}f^{(n+1)}(x)dx &= \left. e^{-ikx}f^{(n)}(x)\right\rvert_{-\infty}^{a^-} + ik \int_{-\infty}^{a} e^{-ikx} f^{(n)}(x)dx \\
        &= e^{-ika}\lim_{x\to a^{-}}f^{(n)}(x) + ik \int_{-\infty}^{a} e^{-ikx} f^{(n)}(x)dx
      \end{align*}
      and similarly
      \begin{align*}
        \int_{a}^{\infty}e^{-ikx}f^{(n+1)}(x)dx &= \left. e^{-ikx}f^{(n)}(x)\right\rvert_{a^+}^{\infty} + ik \int_{a}^{\infty} e^{-ikx} f^{(n)}(x)dx \\
        &= -e^{-ika}\lim_{x\to a^{+}}f^{(n)}(x) + ik \int_{a}^{\infty} e^{-ikx} f^{(n)}(x)dx.
      \end{align*}

      Therefore, combining we have that
      \begin{align*}
        \fourier{f^{(n+1)}}
        &= \frac{1}{\sqrt{2\pi}}\left[\int_{-\infty}^{a}e^{-ikx}f^{(n+1)}(x)dx + \int_{-\infty}^{a}e^{-ikx}f^{(n+1)}(x)dx\right] \\
        &= \frac{ik}{\sqrt{2\pi}}\int_{-\infty}^{\infty}e^{-ikx}f^{(n)}dx - \frac{1}{\sqrt{2\pi}}e^{-ika}\left(\lim_{x\to a^{+}}f^{(n)}(x) - \lim_{x\to a^{-}}f^{(n)}(x)\right) \\
        &= ik \fourier{f^{(n)}(x)} - \frac{1}{\sqrt{2\pi}}e^{-ika}[f^{(n)}]_a.
      \end{align*}

      From our assumption, we then see that
      \begin{align*}
        \fourier{f^{(n+1)}} &= ik \fourier{f^{(n)}(x)} - \frac{1}{\sqrt{2\pi}}e^{-ika}[f^{(n)}]_a \\
        &= ik \left[(ik)^n F(k) - \frac{1}{\sqrt{2\pi}}e^{-ika}\sum_{j=1}^{n} (ik)^{n-j} [f^{(j-1)}]_a\right] - \frac{1}{\sqrt{2\pi}}e^{-ika}[f^{(n)}]_a \\
        &= (ik)^{n+1}F(k) - \frac{1}{\sqrt{2\pi}}e^{-ika}[f^{(n)}]_a - \frac{1}{\sqrt{2\pi}}e^{-ika}\sum_{j=1}^{n} (ik)^{n-j+1} [f^{(j-1)}]_a  \\
        &= (ik)^{n+1}F(k) - \frac{1}{\sqrt{2\pi}}e^{-ika}\sum_{j=1}^{n+1} (ik)^{n+1-j} [f^{(j-1)}]_a .
      \end{align*}
      Therefore, result \eqref{ind_four} holds for $n+1$ and the result is true by induction.
  \end{enumerate}
\end{proof}
\newpage
