\begin{problem}{6}
  Apply the Laplace transform to solve the following diffusion problem
  \begin{align*}
    & \frac{\partial u(x, t)}{\partial t} = K \frac{\partial^2 u(x, t) }{\partial x^2}, \qquad 0 < x < 1, \quad 0 < t, \\
    & u(x, 0) = 0, \qquad 0 < x < 1, \\
    & u(0, t) = f(t), \quad \frac{\partial }{\partial x}\left[u(1, t)\right] = 0, \qquad 0 < t.
  \end{align*}
\end{problem}

\begin{proof}
  We begin by applying the Laplace transform to the first equation in the diffusion problem.
  Doing so yields
  \begin{align*}
    \laplace{\frac{\partial u(x, t)}{\partial t}} = s\bar{u}(x,s) - \bar{u}(x, 0) = K\frac{d^2\bar{u}(x, s)}{dx^2} = \laplace{K \frac{\partial^2 u(x, t) }{\partial x^2}}
  \end{align*}
  From the initial data, we see that this equation reduces to
  \begin{align*}
    s\bar{u}(x,s) = K\frac{d^2\bar{u}(x, s)}{dx^2},
  \end{align*}
  or, equivalently,
  \begin{align*}
    \frac{d^2\bar{u}(x, s)}{dx^2}-\frac{s}{K}\bar{u}(x,s) =0.
  \end{align*}

  The solution to this homogeneous equation is readily seen to be
  \begin{align}\label{sol}
    \bar{u}(x, s) &= b_1 \exp\left(-x\sqrt{\frac{s}{K}}\right) + b_2 \exp\left(x\sqrt{\frac{s}{K}}\right) \notag \\
    &= c_1 \cosh\left(x\sqrt{\frac{s}{K}}\right) + c_2 \sinh\left(x\sqrt{\frac{s}{K}}\right).
  \end{align}
  Note that the transformed boundary conditions are given by
  \begin{align*}
    \bar{u}(0, s) = \bar{f}(s), \quad \left.\frac{d}{dx}\left[\bar{u}(x, s)\right]\right\rvert_{x=1} = 0.
  \end{align*}
  Using \eqref{sol} in conjunction with the transformed boundary data, we see that
  \begin{align*}
    c_1 &= \bar{f}(s)
    c_2 &= \bar{f}(s) \exp\left(-2\sqrt{\frac{s}{K}}\right).
  \end{align*}

  Therefore, the solution to the transformed equation is given by
  \begin{align*}
    \bar{u}(x, s) = \bar{f}(s)\cosh\left(x\sqrt{\frac{s}{K}}\right) + \bar{f}(s) \exp\left(-2\sqrt{\frac{s}{K}}\right)\sinh\left(x\sqrt{\frac{s}{K}}\right).
  \end{align*}
  and the solution to the original equation is given by
  \begin{align*}
    u(x, t) &= \laplaceinv{\bar{u}(x, s)} \\
    &= \laplaceinv{\bar{f}(s)\cosh\left(x\sqrt{\frac{s}{K}}\right) + \bar{f}(s) \exp\left(-2\sqrt{\frac{s}{K}}\right)\sinh\left(x\sqrt{\frac{s}{K}}\right)}.
  \end{align*}
\end{proof}
\newpage
