\begin{problem}{5}
  Solve the following integral equation by the Laplace transform
  \begin{align*}
    f(t) = t\cos at + a \int_0^t f(\tau)\sin a(t-\tau) d\tau.
  \end{align*}
\end{problem}

\begin{proof}
  Let $g(t) = t \cos a t$ and $h(t) = \sin a t$. Then from the definition of the convolution,
  the integral equation is equivalent to
  \begin{align*}
    f(t) = g(t) + a (h \ast f)(t).
  \end{align*}

  From the Convolution Theorem, application of the Laplace transform to this equation yields that
  \begin{align*}
    \laplace{f}(t) = \bar{f}(s) = \bar{g}(s) + a \bar{f}(s)\bar{h}(s) = \laplace{g(t) + a (h \ast f)(t)},
  \end{align*}
  where $\bar{f}(s) = \laplace{f(t)}$, $\bar{g}(s) = \laplace{g(t)}$, and $\bar{h}(s) = \laplace{h(t)}$.
  The resulting equation is an algebraic one; solving for $\bar{f}(s)$ yields that
  \begin{align*}
    \bar{f}(s) = \frac{\bar{g}(s)}{1- a\bar{h}(s)}.
  \end{align*}

  From the table of Laplace transforms, we know that
  \begin{align*}
    \bar{g}(s) = \laplace{t \cos a t} = \frac{s^2 - a^2}{(s^2+a^2)^2}
  \end{align*}
  and
  \begin{align*}
    \bar{h}(s) = \laplace{\sin a t} = \frac{a}{s^2+a^2}.
  \end{align*}
  Thus, we have that
  \begin{align*}
    \bar{f}(s) &= \frac{\bar{g}(s)}{1 -a\bar{h}(s) } \\
    &= \frac{s^2 - a^2}{s^2(s^2 + a^2)}.
  \end{align*}

  Applying the partial fraction decomposition method to this equation, we see that it can be rewritten as
  \begin{align*}
    \bar{f}(s)
    = \frac{s^2 - a^2}{s^2(s^2 + a^2)}
    &= -\frac{1}{s^2} + \frac{2}{s^2+a^2}.
  \end{align*}
  Therefore, by taking the inverse Laplace transform of this equation, we see that
  the solution to the original integral equation is
  \begin{align*}
    f(t) = \laplaceinv{\bar{f}(s)}
    &= -\laplaceinv{\frac{1}{s^2}} + 2\laplaceinv{\frac{1}{s^2+a^2}} \\
    &= -t + \frac{2\sin a t}{a}.
  \end{align*}
\end{proof}
\newpage
