\begin{problem}{8.12}
  Assuming that
  \begin{align*}
    \mellin{f\left(r e^{i \theta}\right)} = \int_0^\infty r^{p-1} f\left(r e^{i \theta}\right) dr
  \end{align*}
  where $p$ is real. Putting $\xi = r e^{i \theta}$ and $\mellin{f(\xi)} = F(p)$, show that
  \begin{enumerate}
    \item[a.] $\mellin{f(r e^{i \theta})} = e^{-ip\theta}F(p)$.
  \end{enumerate}
  Hence, deduce
  \begin{enumerate}
    \item[b.] $\mellininv{F(p) \cos p\theta} = \Re{\{f(r e^{i \theta})\}}$,
    \item[c.] $\mellininv{F(p) \sin p\theta} = -\Im{\{f(r e^{i \theta})\}}.$
  \end{enumerate}

\end{problem}

\begin{proof}
  \begin{enumerate}
    \item[a.] If $\xi = r e^{i \theta}$, then $r = \xi e^{-i \theta}$ and $dr = e^{-i \theta}d \xi $.
      Now, from our assumption, we see that
      \begin{align*}
        \mellin{f\left(r e^{i\theta}\right)}
        &= \int_0^\infty r^{p-1} f\left(r e^{i\theta}\right) dr \\
        &= \int_0^\infty \left(\xi e^{-i \theta}\right)^{p-1} f\left(\xi\right) e^{-i\theta} d\xi \\
        &= e^{-ip\theta} \int_0^\infty \xi^{p-1} f\left(\xi\right) d\xi \\
        &= e^{-ip\theta} F(p),
      \end{align*}
      as desired.

    \item[b.] As shown above, we have that
      \begin{align*}
        \mellin{f(r e^{i \theta})} = e^{-ip\theta}F(p).
      \end{align*}
      From the definition of the complex exponential, this implies that
      \begin{align*}
        \mellin{f(r e^{i \theta})} = e^{-ip\theta}F(p) = F(p)\cos p\theta  -i F(p)\sin p \theta.
      \end{align*}
      Thus, applying the inverse Mellin transform, we see that
      \begin{align}\label{com}
        f(r e^{i \theta}) = \mellininv{F(p)\cos p\theta} -i \mellininv{F(p)\sin p \theta }.
      \end{align}

      Therefore, we have that
      \begin{align*}
        \mellininv{F(p)\cos p\theta } = \Re{\{f(r e^{i \theta})\}}.
      \end{align*}

    \item[c.] Similarly, from \eqref{com}, we have that
      \begin{align*}
        \mellininv{F(p) \sin p\theta} = -\Im{\{f(r e^{i \theta})\}}.
      \end{align*}
  \end{enumerate}
\end{proof}
\newpage
