\begin{problem}{8.4}
  Show that
  \begin{align*}
    \mellin{\frac{1}{(1 + ax)^n}} = \frac{\Gamma(p)\Gamma(n-p)}{a^p \Gamma(n)}.
  \end{align*}
\end{problem}

\begin{proof}
  Let $\displaystyle f(x) = \frac{1}{(1+x)^n}$ where $n > 0$. Recall that the Beta function
  \begin{align*}
    B(x, y) = \int_0^1 t^{x-1}(1-t)^{y-1}dt
  \end{align*}
  satisfies the property that
  \begin{align*}
    B(x, y) = \frac{\Gamma(x)\Gamma(y)}{\Gamma(x+y)}.
  \end{align*}

  From the definition of the Gamma function, we see that
  \begin{align*}
    B(x, y) = \frac{\Gamma(x)\Gamma(y)}{\Gamma(x+y)} = \int_0^\infty \frac{t^{x-1}}{(1+t)^{x+y}} dt.
  \end{align*}
  Thus, we have from the definition of the Mellin transform that
  \begin{align*}
    \mellin{f(x)} &= \int_0^\infty \frac{x^{p-1}}{(1+x)^n} dx\\
    &= \int_0^\infty \frac{x^{p-1}}{(1+x)^{n-p+p}} dx \\
    &= \frac{\Gamma(p)\Gamma(n-p)}{\Gamma(n)}.
  \end{align*}

  Therefore, by the scaling property of the Mellin transform,
  \begin{align*}
    \mellin{\frac{1}{(1 + ax)^n}} = \mellin{f(ax)}
    &= \frac{\mellin{f(x)}}{a^{p}} \\
    &= \frac{\Gamma(p)\Gamma(n-p)}{a^{p}\Gamma(n)}.
  \end{align*}

\end{proof}
\newpage
