\begin{problem}{8.14}
  Use $\displaystyle \mellininv{\frac{\pi}{\sin p\pi}} = \frac{1}{1+x} = f(x)$ and exercise 8.12
  to show that
  \begin{enumerate}
    \item[a.] $\displaystyle \mellininv{\frac{\pi \cos p\theta}{\sin p\pi}} = \frac{1 + r\cos\theta}{1  +2r \cos\theta + r^2}$,
    \item[b.] $\displaystyle \mellininv{\frac{\pi \sin p\theta}{\sin p\pi}} = \frac{r\sin\theta}{1  +2r \cos\theta + r^2}$.
  \end{enumerate}
\end{problem}

\begin{proof}
  Suppose that $\displaystyle F(p) = \frac{\pi}{\sin p\pi}$. Then from our assumption, we have that
  \begin{align*}
    \mellin{f(x)} = \mellin{\frac{1}{1+x}} = \frac{\pi}{\sin p\pi} = F(p).
  \end{align*}

  Now suppose that $x = re^{i\theta}$. Then, from the complex exponential and other properties of complex numbers and trigonometric functions, we have that
  \begin{align*}
    f(re^{i\theta}) = \frac{1}{1+re^{i\theta}} &= \frac{1}{1 + r\cos\theta + ir\sin\theta}\left[\frac{1 + r\cos\theta - ir\sin\theta}{1 + r\cos\theta - ir\sin\theta}\right] \\
    &= \left[\frac{1 + r\cos\theta}{(1 + r\cos\theta)^2 + r^2\sin^2\theta}\right] -i\left[\frac{r\sin\theta}{(1 + r\cos\theta)^2 + r^2\sin^2\theta}\right] \\
    &= \left[\frac{1 + r\cos\theta}{1 + 2r \cos\theta + r^2}\right] -i\left[\frac{r\sin\theta}{1 + 2r \cos\theta + r^2}\right] \\
  \end{align*}
  Thus, we have that
  \begin{subequations}
    \begin{align}
      \Re{\{f(re^{i\theta})\}} &= \frac{1 + r\cos\theta}{1 + 2r \cos\theta + r^2} \label{8.14:real} \\
      \Re{\{f(re^{i\theta})\}} &= -\frac{r\sin\theta}{1 + 2r \cos\theta + r^2} \label{8.14:imag}
    \end{align}
  \end{subequations}

  \begin{enumerate}
    \item[a.] Therefore, we have from \eqref{8.14:real} and exercise 8.12.b that
      \begin{align*}
        \mellininv{\frac{\pi \cos p\theta}{\sin p\pi}} = \mellininv{F(p)\cos p\theta} = \Re{\{f(re^{i\theta})\}} = \frac{1 + r\cos\theta}{1  +2r \cos\theta + r^2}.
      \end{align*}

    \item[b.] Similarly, we see from \eqref{8.14:imag} and exercise 8.12.c that
      \begin{align*}
        \mellininv{\frac{\pi \sin p\theta}{\sin p\pi}} = \mellininv{F(p)\sin p\theta} = -\Im{\{f(re^{i\theta})\}} = \frac{r\sin\theta}{1  +2r \cos\theta + r^2}.
      \end{align*}
  \end{enumerate}
\end{proof}
\newpage
