\begin{problem}{2.47}
  Apply the Fourier transform to solve the equation
  \begin{align*}
    u_{xxxx}+u_{yy} = 0, \qquad -\infty< x < \infty,\ 0 \leq y
  \end{align*}
  satisfying the conditions
  \begin{align*}
    u(x, 0) = f(x), \quad u_y(x,0) = 0, \qquad \text{for $-\infty < x < \infty$}
  \end{align*}
  where $u(x, y)$ and its partial derivatives vanish as $|x| \to \infty$.
\end{problem}

\begin{proof}
  We begin by applying the Fourier transform to the system of differential equations. Using
  the properties of the Fourier transform with respect to $x$, we see that
  \begin{align*}
    &\der{y}{2}\left[U(k, y)\right] + k^4 U(k, y) = 0 \\
    &U(k, 0) = F(k)\\
    &\left. \der{y}{}\left[U(k, y)\right] \right \rvert_{y=0} = 0, \qquad -\infty < k < \infty,\ 0 \leq y.
  \end{align*}
  The first equation of the transformed system is a second-order linear homogeneous ordinary differential equation. Its solution
  is given by
  \begin{align*}
    U(k, y) = c_1 \cos(k^2 y) + c_2  \sin (k^2 y).
  \end{align*}

  From this general solution, we see from the second equation that
  \begin{align*}
    U(k, 0) = c_1 = F(k).
  \end{align*}
  Similarly, using the general solution, we see from the third equation that
  \begin{align*}
    \der{y}{}\left[U(k,y)\right] = -c_1 k^2 \sin(k^2y) + c_2 k^2 \cos(k^2 y)
  \end{align*}
  which implies that
  \begin{align*}
    &\left. \der{y}{}\left[U(k, y)\right] \right \rvert_{y=0} = c_2 k^2 = 0.
  \end{align*}
  Since this must hold for all $k$, we must have have that $c_2 = 0$.

  Thus, the solution to the transformed system is given by
  \begin{align*}
    U(k, y) = F(k)\cos(k^2y).
  \end{align*}
  Therefore, the solution to the original differential equation is
  \begin{align*}
    u(x, y) = \fourierinv{U(k, y)} = \frac{1}{\sqrt{2\pi}}\int_{-\infty}^\infty F(k)\cos(k^2 y) e^{ikx} dk.
  \end{align*}
\end{proof}
\newpage
