\begin{problem}{2.20}
  Apply the Fourier cosine transform to find the solution $u(x, y)$ of the problem
  \begin{align*}
    u_{xx} + u_{yy} = 0 &, \qquad 0 < x < \infty, \quad 0 < y < \infty \\
    u(x, 0) = H(a-x) &, \qquad x < a \\
    u_x(0, y) = 0 &, \qquad 0 < x, y < \infty.
  \end{align*}
\end{problem}

\begin{proof}
  Consider the function $u(x, y)$. The Fourier cosine transform
  of $u$ with respect to $x$ is defined as
  \begin{align*}
    \fouriercos{u(x, y)} = U_c(k, y) = \sqrt{\frac{2}{\pi}} \int_{0}^{\infty}  u(x, y)  \cos (kx)dx.
  \end{align*}
  From this definition we see using the Leibniz integral rule that
  \begin{align*}
    \fouriercos{\frac{\partial^n u(x,y)}{\partial y^n}}
    &= \sqrt{\frac{2}{\pi}} \int_{0}^{\infty} \frac{\partial^n u(x,y)}{\partial y^n} \cos (kx)dx \\
    &= \der{y}{n}\left[\sqrt{\frac{2}{\pi}} \int_{0}^{\infty} u(x,y) \cos (kx)dx\right] \\
    &= \der{y}{n}\left[\fouriercos{u(x,y)}\right].
  \end{align*}
  The transforms of the partials of $u$ with respect to $x$ are not as easy to characterize. Nevertheless,
  we see from the properties of the Fourier cosine transform that
  \begin{align*}
    \fouriercos{\frac{\partial u(x,y)}{\partial x}} = k \fouriersin{u(x,y)} - \sqrt{\frac{2}{\pi}}u(0, y)
  \end{align*}
  and
  \begin{align*}
    \fouriercos{\frac{\partial^2 u(x,y)}{\partial x^2}} = -k^2 \fouriercos{u(x,y)} - \sqrt{\frac{2}{\pi}}u_x(0, y)
  \end{align*}

  Let $U_c(x, y) = \fouriercos{u(x,y)}$. Then, applying the Fourier cosine transform to the first differential equation shows
  that
  \begin{align*}
    \fouriercos{u_{xx} + u_{yy}} = -k^2 U_c(k,y) - \sqrt{\frac{2}{\pi}}u_x(0,y) + \der{y}{2}\left[U_c(k,y)\right] = 0 = \fouriercos{0}.
  \end{align*}
  From the third equation we see that $u_x(0, y) = 0$ for all $0 < x,y < \infty$
  which implies that the above equation reduces to
  \begin{align*}
    \der{y}{2}\left[U_c(k,y)\right] -k^2 U_c(k,y) = 0.
  \end{align*}
  This is a second-order linear homogeneous differential equation, the solution to which is readily seen
  to be
  \begin{align*}
    U_c(k,y) = c_1 e^{-ky} + c_2 e^{k y}.
  \end{align*}
  However, since $U_c(k,y) \to 0$ as $k \to \infty$, we must have that
  $c_2 = 0$. Thus, the solution to the previous differential equation is given by
  \begin{align}\label{costransol}
    U_c(k,y) = c_1 e^{-ky}.
  \end{align}

  We now apply the Fourier cosine transform to the second differential equation yielding
  \begin{align*}
    \fouriercos{u(x, 0)} = U_c(k, 0) = \fouriercos{H(a-x)}.
  \end{align*}
  Using the form \eqref{costransol} of the solution to the transformed differential equation
  and a table of Fourier cosine transforms we see that
  \begin{align*}
    U_c(k,0) = c_1 = \fouriercos{H(a-x)} = \sqrt{\frac{2}{\pi}}\left(\frac{\sin ak}{k}\right).
  \end{align*}
  Thus, the solution to the transformed differential equation with the boundary conditions listed above is given by
  \begin{align*}
    U_c(k, y) = \fouriercos{H(a-x)}e^{-ky} = \sqrt{\frac{2}{\pi}}\left(\frac{\sin ak}{k}\right)e^{-ky}.
  \end{align*}

  Therefore, taking the inverse Fourier cosine transform to both sides shows that
  the solution to the original differential equation is given by
  \begin{align*}
    u(x, y) = \fouriercosinv{U_c(k, y)}
    &= \sqrt{\frac{2}{\pi}} \int_0^\infty \sqrt{\frac{2}{\pi}}\left(\frac{\sin ak}{k}\right)e^{-ky} \cos kx dk \\
    &= \frac{2}{\pi} \int_0^\infty \left(\frac{\sin ak}{k}\right)e^{-ky} \cos kx dk.
  \end{align*}

\end{proof}
\newpage
