\begin{problem}{3.24}
  Suppose that $\laplace{f(t)} = \bar{f}(s)$ and $\laplace{g(x, t)} = \bar{h}(s)\exp(-x\bar{h}(s))$. Prove that:
  \begin{enumerate}
    \item[a.] $\displaystyle \laplace{\int_0^\infty g(x, t)f(x) dx} = \bar{h}(s)\bar{f}(\bar{h}(s))$.
  \end{enumerate}
\end{problem}

\begin{proof}
  \begin{enumerate}
    \item[a.] From the definition of the Laplace transform, we have that
      \begin{align*}
        \laplace{\int_0^\infty g(x,t) f(x) dx} = \int_0^\infty\left[\int_0^\infty g(x,t) f(x) dx\right]e^{-st}dt.
      \end{align*}

      Interchanging the order of integration yields that
      \begin{align*}
        \laplace{\int_0^\infty g(x,t) f(x) dx} &= \int_0^\infty\left[\int_0^\infty g(x,t) f(x) dx\right]e^{-st}dt \\
        &= \int_0^\infty f(x) \left[\int_0^\infty g(x,t) e^{-st}dt\right]dx \\
        &= \int_0^\infty f(x) \laplace{g(x, t)}dx.
      \end{align*}

      From the relation $\laplace{g(x, t)} = \bar{h}(s)\exp(-x\bar{h}(s))$, we thus see that
      \begin{align*}
        \laplace{\int_0^\infty g(x,t) f(x) dx} &= \int_0^\infty f(x) \laplace{g(x, t)}dx \\
        &= \int_0^\infty f(x) \bar{h}(s) \exp(-x\bar{h}(s))dx.
      \end{align*}

      Using the definition of the Laplace transform, we see that
      \begin{align*}
        \bar{f}(\bar{h}(s)) = \int_0^\infty f(t) \exp(-\bar{h}(s)t) dt.
      \end{align*}

      Therefore,
      \begin{align*}
        \laplace{\int_0^\infty g(x,t) f(x) dx}
        &= \int_0^\infty f(x) \bar{h}(s) \exp(-x\bar{h}(s))dx \\
        &= \bar{h}(s)\int_0^\infty f(x) \exp(-x\bar{h}(s))dx \\
        &= \bar{h}(s) \bar{f}(\bar{h}(s)).
      \end{align*}
      and we are done.
  \end{enumerate}
\end{proof}
\newpage
