\begin{problem}{3.23}
  Show that:
  \begin{enumerate}
    \item[a.] $\displaystyle \laplace{t \cos(at) e^{-bt}} = \frac{(s+b)^2 - a^2}{\left[(s+b)^2+a^2\right]^2}.$
  \end{enumerate}
\end{problem}

\begin{proof}
  \begin{enumerate}
    \item[a.] Let $f(t) = t \cos(at)$ and suppose that $\bar{f}(s) = \laplace{f(t)}$.

      As shown previously, we know that
      \begin{align*}
        \bar{f}(s) = \laplace{f(t)} = \laplace{t \cos(at)} = \frac{s^2 - a^2}{(s^2+a^2)^2}.
      \end{align*}

      Therefore, by Heaviside's First Shifting Theorem,
      \begin{align*}
        \laplace{t\cos (at) e^{-bt}} = \laplace{f(t)e^{-bt}} = \bar{f}(s+b) = \frac{(s+b)^2 - a^2}{\left[(s+b)^2+a^2\right]^2},
      \end{align*}
      and we are done.
  \end{enumerate}
\end{proof}
\newpage
