\begin{problem}{3.32}
  Use Heaviside's Second Shifting Theorem to obtain the Laplace transforms of the
  following functions:
  \begin{enumerate}
    \item[a.] $f(t) = (t-a)^n H(t-a)$,
    \item[e.] $f(t) = \cos 2t H(t-\pi)$.
  \end{enumerate}
\end{problem}

\begin{proof}
  Heaviside's Second Shifting Theorem states that if $\laplace{f(t)} = \bar{f}(s)$, then
  \begin{align}
    \laplace{f(t-a)H(t - a)} = e^{-as}\bar{f}(s) \label{hvs:1}
  \end{align}
  or, equivalently,
  \begin{align}
    \laplace{f(t)H(t - a)} = e^{-as}\laplace{f(t+a)} \label{hvs:2}.
  \end{align}
  \begin{enumerate}
    \item[a.] Let $g(t) = t^n$. Then $f(t) = g(t-a)H(t-a)$ and from our table
      of Laplace transforms,
      \begin{align*}
        \bar{g}(s) = \laplace{g(t)} = \laplace{t^n} = \frac{n!}{s^{n+1}}.
      \end{align*}
      Therefore, from \eqref{hvs:1}, we see that
      \begin{align*}
        \laplace{f(t)} = \laplace{g(t-a)H(t-a)} = e^{-as}\bar{g}(s) = \frac{n!e^{-as}}{s^{n+1}}.
      \end{align*}
    \item[e.] Let $g(t) = \cos 2t$. Then $f(t) = g(t)H(t-\pi)$ and from
      \eqref{hvs:2}, we see that
      \begin{align*}
        \laplace{f(t)} = \laplace{g(t)H(t-\pi)} = e^{-\pi s} \laplace{g(t+\pi)}.
      \end{align*}
      Note that
      \begin{align*}
        \laplace{g(t+\pi)} = \laplace{\cos 2(t+\pi)} = \laplace{\cos 2 t} = \frac{s}{s^2+4}.
      \end{align*}
      Therefore,
      \begin{align*}
        \laplace{f(t)} = e^{-\pi s} \laplace{g(t+\pi)} = \frac{se^{-\pi s}}{s^2+4}.
      \end{align*}
  \end{enumerate}

\end{proof}
\newpage
