\begin{problem}{4.40}
  Solve the telegraph equation
  \begin{align*}
    &u_{tt} - c^2 u_{xx} + 2a u_t = 0, \qquad -\infty < x < \infty, \quad 0 < t \\
    & u(x, 0) = 0, \quad u_t(x,0) = g(x).
  \end{align*}
\end{problem}

\begin{proof}
  % We begin by applying the Fourier transform with respect to $x$ to the differential equation. Doing so,
  % using previous properties of the Fourier transform, we have that
  % \begin{align*}
  %   \der{t}{2}\left[U(k, t)\right] + 2a \der{t}{}\left[U(k, t)\right] + c^2k^2 U(k, t) = 0,
  % \end{align*}
  % with the transformed conditions
  % \begin{align*}
  %   U(k, 0) &= 0 \\
  %   \der{t}{}\left[U(k, t)\right] &= G(k).
  % \end{align*}

  % Now, the transformed equation is a second-order linear homogeneous differential equation with constant
  % coefficients, the solution of which is readily seen to be
  % \begin{align*}
  % \end{align*}

  We begin by applying the Laplace transform
  to the equation. Doing so yields
  \begin{align*}
    s^2\bar{u}(x, s) -su(x, 0) - u_t(x, 0) -c^2 \frac{d^2}{dx^2}\left[\bar{u}(x, s)\right] + 2as\bar{u}(x, s) - 2au(x, 0) = 0.
  \end{align*}
  Using the initial data, this equation reduces to
  \begin{align*}
    s^2\bar{u}(x, s) - g(x) -c^2 \frac{d^2}{dx^2}\left[\bar{u}(x, s)\right] + 2as\bar{u}(s) = 0,
  \end{align*}
  or, equivalently,
  \begin{align*}
    \frac{d^2}{dx^2}\left[\bar{u}(x, s)\right] - \frac{s^2 + 2as}{c^2}\bar{u}(x, s)= -\frac{g(x)}{c^2}.
  \end{align*}

  Now, applying the Fourier transform to this equation yields
  \begin{align*}
    k^2 \bar{U}(k, s) + \frac{s^2 + 2as}{c^2}\bar{U}(k, s)= \frac{G(k)}{c^2}.
  \end{align*}
  Solving the resulting algebraic equation for $\bar{U}(k, s)$ shows that
  \begin{align*}
    \bar{U}(k, s) = \frac{G(k)}{s^2 + 2as + k^2c^2} = \frac{G(k)}{(s+ a)^2 + k^2c^2- a^2 }.
  \end{align*}
  From our table of Laplace transforms, we see that
  \begin{align*}
    \laplace{e^{at}\sin bt} = \frac{b}{(s-a)^2+b^2}.
  \end{align*}

  Thus, the inverse Laplace transform of the above equation is
  \begin{align*}
    U(k, t) = \laplaceinv{\bar{U}(k, s)} &= \laplaceinv{\frac{G(k)}{(s+ a)^2 + k^2c^2- a^2 }} \\
    &= G(k)\frac{e^{-at}\sin\left(t\sqrt{k^2c^2-a^2} \right)}{\sqrt{k^2c^2-a^2}}.
  \end{align*}
  Let $\omega(k) = \sqrt{k^2c^2-a^2}$. Then the above equation becomes
  \begin{align*}
    U(k, t) &= G(k)\frac{e^{-at}\sin\left(t\sqrt{k^2c^2-a^2} \right)}{\sqrt{k^2c^2-a^2}} \\
    &= G(k)\frac{e^{-at}\sin\left(\omega(k) t\right)}{\omega(k)} \\
    &= e^{-at}G(k)F(k, t),
  \end{align*}
  where
  \begin{align*}
    F(k, t) = \frac{\sin\left(\omega(k) t\right)}{\omega(k)}.
  \end{align*}

  Therefore, according to the Convolution Theorem, the solution to the original equation is
  \begin{align*}
    u(x, t) = \fourierinv{U(k, t)} &= e^{-at}\fourierinv{G(k)F(k, t)} \\
    &= e^{-at}\left[ g(x) \ast f(x, t) \right]\\
    &= \frac{e^{-at}}{\sqrt{2\pi}} \int_{-\infty}^\infty g(\xi)f(x-\xi, t) d\xi.
  \end{align*}
\end{proof}
\newpage
