\begin{problem}{4.37}
  Show that the solution of the differential difference equation
  \begin{align*}
    \der{t}{}u(t) - u(t-1) = 2, \qquad u(0) = 0
  \end{align*}
  is
  \begin{align*}
    u(t) = 2 \left[t - \frac{(t-1)^2}{2!} + \frac{(t-2)^3}{3!} + \dots + \frac{(t-n)^{n+1}}{(n+1)!}\right], \quad t > n
  \end{align*}
\end{problem}

\begin{proof}
  Applying the Laplace transform to the differential difference equation yields
  that
  \begin{align*}
    s\bar{u}(s) - u(0) - e^{-s}\left[\bar{u}(s) - u(0)\bar{S}_0(s)\right] = \frac{2}{s}
  \end{align*}
  In light of the initial data, this equation reduces to
  \begin{align*}
    s\bar{u}(s) - e^{-s}\bar{u}(s) = \frac{2}{s},
  \end{align*}
  or, equivalently,
  \begin{align*}
    \bar{u}(s) = \frac{2}{s(s-e^{s})} = \frac{2}{s^2}\left(1 - \frac{e^{-s}}{s}\right)^{-1}
  \end{align*}

  Expanding the right term in terms of its power series we see that
  \begin{align*}
    \bar{u}(s)
    &= \frac{2}{s^2}\left(1 - \frac{e^{-s}}{s}\right)^{-1}\\
    &= \frac{2}{s^2}\sum_{n=0}^\infty \frac{e^{-ns}}{s^n}\\
    &= 2\sum_{n=0}^\infty \frac{e^{-ns}}{s^{n+2}}.
  \end{align*}

  Recall that
  \begin{align*}
    \laplaceinv{\frac{e^{-as}}{s^n}} = \frac{(t-a)^{n-1}}{\Gamma(n)}H(t-a).
  \end{align*}

  Therefore, the solution to the original differential difference equation is
  \begin{align*}
    u(t) &= \laplaceinv{2\sum_{n=0}^\infty \frac{e^{-ns}}{s^{n+2}} }\\
    &= 2\sum_{n=0}^\infty \laplaceinv{\frac{e^{-ns}}{s^{n+2}}} \\
    &= 2\sum_{n=0}^\infty \frac{(t-n)^{n+1}}{\Gamma(n+2)}H(t-n) \\
    &= 2\sum_{n=0}^\infty \frac{(t-n)^{n+1}}{(n+1)!}H(t-n).
  \end{align*}

\end{proof}
\newpage
