\begin{problem}{4.29}
  Show that
  \begin{enumerate}
    \item  [b.]$\displaystyle I(a) = \int_0^{\infty} e^{-ax}\left(\frac{\sin qx - \sin px}{x}\right)dx = \tan^{-1}\left(\frac{q}{a}\right) - \tan^{-1}\left(\frac{p}{a}\right)$
  \end{enumerate}
\end{problem}

\begin{proof}
  \begin{enumerate}
    \item[b.]
      Let $f(x) = \sin qx - \sin px$ and $\displaystyle g(x) = \frac{f(x)}{x}$.

      From the definition of the Laplace transform, we see that this integral is the Laplace transform of
      $\displaystyle \frac{f(x)}{x}$ with respect to $x$ in the variable $a$, i.e.
      \begin{align*}
        I(a) = \int_0^{\infty} e^{-ax}\left(\frac{\sin qx - \sin px}{x}\right)dx = \laplace{\frac{f(x)}{x}} = \bar{g}(a).
      \end{align*}

      From a previous result, we know that
      \begin{align*}
        I(a) = \laplace{\frac{f(x)}{x}} = \int_a^\infty \bar{f}(a) da
      \end{align*}
      where $\bar{f}(a) = \laplace{f(x)}$. Our table of Laplace transforms shows that
      \begin{align*}
        \bar{f}(a) = \laplace{f(x)} &= \laplace{\sin qx - \sin px} \\
        &= \frac{q}{a^2 + q^2} - \frac{p}{a^2 + p^2}.
      \end{align*}

      Thus, we see that
      \begin{align*}
        I(a) = \int_a^\infty \bar{f}(a) da &= \int_a^\infty \frac{q}{a^2 + q^2} - \frac{p}{a^2 + p^2} da.
      \end{align*}
      Recall that
      \begin{align*}
        \int \frac{t}{a^2 + t^2}da = \tan^{-1}\left(\frac{a}{t}\right) + C.
      \end{align*}
      Therefore, we have that
      \begin{align*}
        I(a) &= \int_a^\infty \frac{q}{a^2 + q^2} - \frac{p}{a^2 + p^2} da \\
        &= \left[\frac{\pi}{2} - \tan^{-1}\left(\frac{a}{q}\right)\right] - \left[\frac{\pi}{2} - \tan^{-1}\left(\frac{a}{p}\right)\right] \\
        &= \tan^{-1}\left(\frac{q}{a}\right) - \tan^{-1}\left(\frac{p}{a}\right).
      \end{align*}

  \end{enumerate}
\end{proof}
\newpage
