\begin{problem}{8.2.2}
  If $Sf(x)$ is the Schwarzian derivative of $f(x)$ with $f \in C^3$ and
  $\displaystyle F(x) = \frac{f''(x)}{f'(x)}$, show that
  $Sf(x) = F'(x) - (F(x))^2/2$.
\end{problem}

\begin{proof}
  Recall that the Schwarzian derivative of $f$ is given by
  \begin{align*}
    Sf(x) = \frac{f'''(x)}{f'(x)} - \frac{3}{2}\left[\frac{f''(x)}{f'(x)}\right]^2.
  \end{align*}

  We readily see from the definition of $F(x)$ that
  \begin{align*}
    F'(x) - \frac{1}{2}\left[F(x)\right]^2
    &= \frac{f'(x)f'''(x) - f''(x)^2}{f'(x)^2} - \frac{1}{2}\left[\frac{f''(x)}{f'(x)}\right]^2 \\
    &= \frac{f'''(x)}{f'(x)} - \frac{3}{2}\left[\frac{f''(x)}{f'(x)}\right]^2 \\
    &= Sf(x)
  \end{align*}
  and we are done.
\end{proof}
\newpage
