\begin{problem}{6}
  Evaluate the following definite integrals:
  \begin{enumerate}
    \item[a.] $\displaystyle \int_0^\infty \frac{\sin ax \sin bx}{x^2} dx,$
    \item[b.] $\displaystyle \int_0^\infty \frac{(a^2 - x^2)^2}{(x^2+a^2)^4} dx, \quad a >0$.
  \end{enumerate}
\end{problem}

\begin{proof}
  Suppose that $F_c(k) = \fouriercos{f(x)}$ and $G_c(k) = \fouriercos{g(x)}$. Then Parseval's
  relation derived from the Convolution Theorem for the Fourier Cosine Transform states
  that
  \begin{align}\label{parseval}
    \int_{0}^\infty F_c(k)G_c(k) dk = \int_0^\infty f(x)g(x) dx.
  \end{align}
  \begin{enumerate}
    \item[a.] Let $\displaystyle F_c(k) = \frac{\sin a k}{k}$ and $\displaystyle G_c(k) = \frac{\sin b k}{k}$.
      Then Parseval's theorem shows that
      \begin{align*}
        \int_0^\infty \frac{\sin ak \sin bk}{k^2} dk = \int_0^\infty F_c(k)G_c(k)dk = \int_0^\infty f(x)g(x)dx
      \end{align*}
      where $f(x) = \fouriercosinv{F_c(k)}$ and $f(x) = \fouriercosinv{G_c(k)}$. From our table
      of Fourier Cosine Transforms, we see that for $p\in\mathbb{R}$,
      \begin{align*}
        \fouriercos{H(p-x)} = \sqrt{\frac{2}{\pi}}\frac{\sin p k }{k}.
      \end{align*}
      This implies that
      \begin{align*}
        \fouriercosinv{\frac{\sin p k }{k}} = \sqrt{\frac{\pi}{2}}H(p-x).
      \end{align*}
      Thus, we have that
      \begin{align*}
        \int_0^\infty \frac{\sin ak \sin bk}{k^2} dk = \int_0^\infty F_c(k)G_c(k)dk = \frac{\pi}{2}\int_0^\infty H(a-x)H(b-x)dx.
      \end{align*}
      Now, we note from the definition of the Heaviside function that
      \begin{align*}
        H(a-x)H(b-x) = \begin{cases}1 & \text{if $x<\min(a,b)$} \\
        0 & \text{if $x>\min(a,b)$} \end{cases}.
      \end{align*}
      Therefore, we have that
      \begin{align*}
        \int_0^\infty \frac{\sin ak \sin bk}{k^2} dk = \frac{\pi}{2}\int_0^\infty H(a-x)H(b-x)dx = \frac{\pi}{2}\int_0^{\min(a,b)}dx = \frac{\pi}{2}\min(a,b).
      \end{align*}

    \item[b.] Let $\displaystyle F_c(k) = \frac{a^2-k^2}{(k^2+a^2)^2}$.
      Then Parseval's theorem shows that
      \begin{align*}
        \int_0^\infty \frac{(a^2 - k^2)^2}{(k^2+a^2)^4} dk = \int_0^\infty F_c(k)F_c(k)dk = \int_0^\infty f(x)f(x)dx
      \end{align*}
      where $f(x) = \fouriercosinv{F_c(k)}$. From our table
      of Fourier Cosine Transforms, we see that for $a > 0$,
      \begin{align*}
        \fouriercos{x e^{-a x}} = \sqrt{\frac{2}{\pi}}\frac{a^2-k^2}{(k^2+a^2)^2}.
      \end{align*}
      This implies that
      \begin{align*}
        \fouriercosinv{\frac{a^2-k^2}{(k^2+a^2)^2}} = \sqrt{\frac{\pi}{2}}.
      \end{align*}

      Thus, we have that
      \begin{align*}
        \int_0^\infty \frac{(a^2 - k^2)^2}{(k^2+a^2)^4} dk = \int_0^\infty F_c(k)F_c(k)dk = \frac{\pi}{2}\int_0^\infty x^2e^{-2ax}dx.
      \end{align*}
      From \eqref{intform}, we see by setting $b = 2a$ and $k=0$ that
      \begin{align*}
        \int_0^\infty x^2e^{-2ax}dx = \frac{1}{4a^3}.
      \end{align*}

      Therefore, we have that
      \begin{align*}
        \int_0^\infty \frac{(a^2 - k^2)^2}{(k^2+a^2)^4} dk = \frac{\pi}{2}\int_0^\infty x^2e^{-2ax}dx = \frac{\pi}{(2a)^3}.
      \end{align*}
  \end{enumerate}
\end{proof}
\newpage
