\begin{problem}{2}
  Find the Laplace Transforms of the following functions:
  \begin{enumerate}
    \item[a.] $\displaystyle f(t) = \int_0^t \frac{\sin ax}{x} dx$,
    \item[b.] $f(t) = t H(t-a)$.
  \end{enumerate}
\end{problem}

\begin{proof}
  Recall that if $f(t) \in L^1(\mathbb{R})$, then the Laplace Transform of $f$ is
  defined to be
  \begin{align}\label{laplacedef}
    \laplace{f(t)} = \bar{f}(s) = \int_0^\infty f(t) e^{-st} dt, \quad \text{Re } s > 0.
  \end{align}
  Note that it can be shown that the Laplace transform satisfies the important
  property
  \begin{align}\label{laplace1}
    \laplace{t^n f(t)} = (-1)^n \der{s}{n}\left[\laplace{f(t)}\right].
  \end{align}
  \begin{enumerate}
    \item[a.] Let $\displaystyle f(t) = \int_0^t \frac{\sin ax}{x} dx$. Then $f(0) = 0$
      and $\displaystyle f'(t) = \frac{\sin at}{t}$ so that $tf'(t) = \sin at$.
      This implies that
      \begin{align*}
        \laplace{tf'(t)} = \laplace{\sin at} = \frac{a}{s^2+a^2}.
      \end{align*}

      The Laplace transform satisfies the following property that relates a function's
      derivative to its Laplace Transform:
      \begin{align*}
        \laplace{f'(t)} = s \laplace{f(t)} - f(0).
      \end{align*}
      This combined with \eqref{laplace1} shows that
      \begin{align*}
        \laplace{tf'(t)} = -\der{s}{}\left[\laplace{f'(t)}\right] = -\der{s}{}\left[s\laplace{f(t)} - f(0)\right] = \frac{a}{s^2+a^2},
      \end{align*}
      or that
      \begin{align*}
        \der{s}{}\left[s \laplace{f(t)}\right] = -\frac{a}{s^2+a^2}.
      \end{align*}
      Integrating both sides of the above equation yields that
      \begin{align*}
        s\laplace{f(t)} = -\int \frac{a}{s^2+a^2} ds = - \tan^{-1}(s/a) + C.
      \end{align*}
      In order to determine the constant of integration, we use the Initial Value Theorem which states
      that
      \begin{align*}
        \lim_{s\to\infty} s \laplace{f(t)} = \lim_{t\to0} f(t) = f(0).
      \end{align*}
      Since $f(0) = 0$, this implies that
      \begin{align*}
        \lim_{s\to\infty} s \laplace{f(t)} = \lim_{s\to\infty} \left[- \tan^{-1}(s/a) + C\right] = 0
      \end{align*}
      or that $C = \frac{\pi}{2}$. Therefore, we have that
      \begin{align*}
        s\laplace{f(t)} = - \tan^{-1}(s/a) + \frac{\pi}{2} = \tan^{-1}(a/s)
      \end{align*}
      so that
      \begin{align*}
        \laplace{f(t)} = \frac{\tan^{-1}(a/s)}{s}.
      \end{align*}

    \item[b.] Let $f(t) = t H(t-a)$ and assume that $a>0$. By property \eqref{laplace1}
      we see that
      \begin{align*}
        \laplace{t H(t-a)} = -\der{s}{}\left[\laplace{H(t-a)}\right].
      \end{align*}
      From our table of Laplace Transforms, we have that
      \begin{align*}
        \laplace{H(t-a)} = \frac{e^{-a s}}{s},
      \end{align*}
      assuming that $a>0$. Therefore,
      \begin{align*}
        \laplace{f(t)} = - \der{s}{}\left[\laplace{H(t-a)}\right] &= - \der{s}{}\left[s^{-1}e^{-as}\right] \\
        &= -\left[-s^{-2}e^{-as} - as^{-1}e^{-as}\right] \\
        &= \frac{(1 + as)e^{-as}}{s^2}.
      \end{align*}
  \end{enumerate}
\end{proof}
\newpage
