\begin{problem}{1}
  Find the Fourier Transforms of the following functions:
  \begin{enumerate}
    \item[a.] $f(x) = x^2 e^{-a|x|}$, $a > 0$,
    \item[b.] $\displaystyle f(x) = \left(1 - \frac{|x|}{2}\right)H\left(1 - \frac{|x|}{2}\right)$.
  \end{enumerate}
\end{problem}

\begin{proof}
  Recall that if $f(x) \in L^1(\mathbb{R})$, then the Fourier Transform of $f$ is
  defined to be
  \begin{align}\label{fourierdef}
    \fourier{f(x)} = F(k) = \frac{1}{\sqrt{2\pi}}\int_{-\infty}^\infty f(x) e^{-ikx} dx.
  \end{align}
  \begin{enumerate}
    \item[a.] If $f(x) = x^2 e^{-a|x|}$, $a > 0$, we see from \eqref{fourierdef}
      that, by definition, the Fourier Transform of $f$ is given by
      \begin{align*}
        \fourier{f(x)} = F(k) &= \frac{1}{\sqrt{2\pi}}\int_{-\infty}^\infty x^2 e^{-a|x|} e^{-ikx} dx \\
        &= \frac{1}{\sqrt{2\pi}}\left[\int_{-\infty}^0 x^2 e^{-(-a+ik)x} dx + \int_{0}^\infty x^2 e^{-(a+ik)x} dx\right].
      \end{align*}
      Now, we see by integration by parts that
      \begin{align*}
        \int_c^d x^2 e^{-(b+ik)x}dx
        &= \left.-\frac{x^2}{b+ik}e^{-(b+ik)x}\right\rvert_c^d + \frac{2}{b+ik}\int_c^d x e^{-(b+ik)x}dx \\
        &= \left.-\frac{x^2}{b+ik}e^{-(b+ik)x}\right\rvert_c^d + \frac{2}{b+ik}\left[\left.-\frac{x}{b+ik}e^{-(b+ik)x}\right\rvert_c^d + \frac{1}{b+ik}\int_c^d e^{-(b+ik)x}dx\right]\\
        &=\left.-\frac{x^2}{b+ik}e^{-(b+ik)x}\right\rvert_c^d + \frac{2}{b+ik}\left[\left.-\frac{x}{b+ik}e^{-(b+ik)x}\right\rvert_c^d - \left.\frac{1}{(b+ik)^2}e^{-(b+ik)x}\right\rvert_c^d\right].
      \end{align*}
      Thus,
      \begin{align*}
        \int_{-\infty}^0 x^2 e^{-(-a+ik)x} dx = -\frac{2}{(-a+ik)^3}
      \end{align*}
      and
      \begin{align*}
        \int_{0}^\infty x^2 e^{-(a+ik)x} dx = \frac{2}{(a+ik)^3}.
      \end{align*}
      Therefore,
      \begin{align*}
        \fourier{f(x)} = F(k)
        &= \frac{1}{\sqrt{2\pi}}\left[\int_{-\infty}^0 x^2 e^{-(-a+ik)x} dx + \int_{0}^\infty x^2 e^{-(a+ik)x} dx\right]\\
        &= \frac{1}{\sqrt{2\pi}}\left[-\frac{2}{(-a+ik)^3} + \frac{2}{(a+ik)^3}\right] \\
        &= \frac{1}{\sqrt{2\pi}}\left[\frac{4a(a^2-3k)}{(a^2+k^2)^3}\right] \\
        &= \sqrt{\frac{2}{\pi}}\left[\frac{2a(a^2-3k)}{(a^2+k^2)^3}\right].
      \end{align*}
    \item[b.] Recall that the Heaviside function $H$ is defined as
      \begin{align*}
        H(x) = \begin{cases}
          1 & \text{if $x > 0$}\\
          0 & \text{if $x < 0$}.
        \end{cases}
      \end{align*}
      Thus,
      \begin{align*}
        H\left(1-\frac{|x|}{2}\right) = \begin{cases}
          1 & \text{if $|x| < 2$}\\
          0 & \text{if $|x| > 2$}.
        \end{cases}
      \end{align*}

      If $\displaystyle f(x) = \left(1 - \frac{|x|}{2}\right)H\left(1 - \frac{|x|}{2}\right)$, we see from \eqref{fourierdef}
      that, by definition, the Fourier Transform of $f$ is given by
      \begin{align*}
        \fourier{f(x)} = F(k)
        &= \frac{1}{\sqrt{2\pi}}\int_{-\infty}^\infty\left(1 - \frac{|x|}{2}\right)H\left(1 - \frac{|x|}{2}\right) e^{-ikx} dx \\
        &= \frac{1}{\sqrt{2\pi}}\int_{-2}^2\left(1 - \frac{|x|}{2}\right)e^{-ikx} dx \\
        &= \frac{1}{\sqrt{2\pi}}\left[\int_{-2}^0 \left(1 + \frac{x}{2}\right) e^{-ikx}dx + \int_{0}^2 \left(1 - \frac{x}{2}\right)e^{-ikx} dx\right].
      \end{align*}
      Now, we see by integration by parts that
      \begin{align*}
        \int_c^d \left(1 \pm \frac{x}{2}\right) e^{-ikx}dx
        &= \left.\frac{i}{k}e^{-ikx}\right\rvert_c^d \pm \frac{1}{2}\int_c^d x e^{-ikx}dx \\
        &= \left.\frac{i}{k}e^{-ikx}\right\rvert_c^d \pm \frac{1}{2}\left[\left.\frac{ix}{k}e^{-ikx} \right\rvert_c^d - \frac{i}{k}\int_c^d e^{-ikx}dx\right] \\
        &= \left.\frac{i}{k}e^{-ikx}\right\rvert_c^d \pm \frac{1}{2}\left[\left.\frac{ix}{k}e^{-ikx} \right\rvert_c^d + \left.\frac{e^{-ikx}}{k^2} \right\rvert_c^d\right].
      \end{align*}
      Thus,
      \begin{align*}
        \int_{-2}^0 \left(1 + \frac{x}{2}\right) e^{-ikx}dx = \frac{1-e^{2ik}+2ik}{2k^2}
      \end{align*}
      and
      \begin{align*}
        \int_{0}^2 \left(1 - \frac{x}{2}\right) e^{-ikx}dx = \frac{1-e^{-2ik}-2ik}{2k^2}
      \end{align*}
      Therefore, using the definition of the complex exponential
      and various trigonometric identities, we have that
      \begin{align*}
        \fourier{f(x)} = F(k)
        &= \frac{1}{\sqrt{2\pi}}\left[\int_{-2}^0 \left(1 + \frac{x}{2}\right) e^{-ikx}dx + \int_{0}^2 \left(1 - \frac{x}{2}\right)e^{-ikx} dx\right] \\
        &= \frac{1}{\sqrt{2\pi}}\left[\frac{1-e^{2ik}+2ik}{2k^2} + \frac{1-e^{-2ik}-2ik}{2k^2} \right] \\
        &= \frac{1}{\sqrt{2\pi}}\left[\frac{1}{k^2} - \frac{e^{-2ik}+e^{2ik}}{2k^2} \right]\\
        &= \frac{1}{\sqrt{2\pi}}\left[\frac{1-\cos 2k}{k^2}\right] \\
        &= \frac{1}{\sqrt{2\pi}}\left[\frac{1-(\cos^2 k - \sin^2 k)}{k^2}\right] \\
        &= \frac{2\sin^2 k}{\sqrt{2\pi} k^2}.
       \end{align*}
  \end{enumerate}
\end{proof}
\newpage
