\begin{problem}{3.6}
  Show that
  \begin{align*}
    \laplace{\int_0^t \frac{f(u)}{u} du} = \frac{1}{s} \int_s^\infty \bar{f}(x) dx.
  \end{align*}
\end{problem}

\begin{proof}
  From the definition of the Laplace transform we see that
  \begin{align*}
    \laplace{\int_0^t \frac{f(u)}{u} du} = \int_0^\infty e^{-st} \left[\int_0^t \frac{f(u)}{u} du\right]dt.
  \end{align*}
  Interchanging the order of integration from $u$ to $t$ where $0 \leq t < \infty$,
  we see that $u \leq t < \infty$ as $0 \leq u < \infty$ and
  \begin{align*}
    \laplace{\int_0^t \frac{f(u)}{u} du} &= \int_0^\infty e^{-st} \left[\int_0^t \frac{f(u)}{u} du\right]dt \\
    &= \int_0^\infty \frac{f(u)}{u}  \left[\int_u^\infty e^{-st}dt\right]du \\
    &= \frac{1}{s} \int_0^\infty \frac{f(u)}{u} e^{-su} du.
  \end{align*}

  We note that $\displaystyle \der{s}{}\left[\frac{e^{-su}}{u}\right] = -e^{-su}$
  so that in particular we have that
  \begin{align*}
    - \int_s^\infty e^{-su} ds = \left.-\frac{e^{-su}}{u}\right\rvert_s^\infty = -\frac{e^{-su}}{u}
  \end{align*}
  or that
  \begin{align*}
    \int_s^\infty e^{-su} ds = \frac{e^{-su}}{u}.
  \end{align*}
  Thus,
  \begin{align*}
    \laplace{\int_0^t \frac{f(u)}{u} du}
    &= \frac{1}{s} \int_0^\infty \frac{f(u)}{u} e^{-su} du \\
    &= \frac{1}{s}\int_0^\infty f(u)\left[\int_s^\infty e^{-su} ds \right]du.
  \end{align*}

  Interchanging the order of integration yet again from $s$ to $u$ where $s \leq s < \infty$
  as $0 \leq u < \infty$, we see that the integration limits remain unchanged and therefore
  that
  \begin{align*}
    \laplace{\int_0^t \frac{f(u)}{u} du}
    &= \frac{1}{s}\int_0^\infty f(u) \left[\int_s^\infty e^{-su} ds\right] du \\
    &= \frac{1}{s}\int_s^\infty \left[\int_0^\infty f(u)e^{-su} du\right] ds \\
    &= \frac{1}{s}\int_s^\infty \bar{f}(s) ds \\
    &= \frac{1}{s}\int_s^\infty \bar{f}(x) dx,
  \end{align*}
  and we are done.

\end{proof}
\newpage
