\begin{problem}{3.15}
  Show that
  \begin{enumerate}
    \item[b.] $\displaystyle \laplace{t^n e^{at}} = \frac{n!}{(s-a)^{n+1}}$.
  \end{enumerate}
\end{problem}

\begin{proof}
  \begin{enumerate}
    \item[b.]
      Let $f(t) = t^n$. By Heaviside's First Shifting Theorem, we have that
      \begin{align*}
        \laplace{t^n e^{at}} = \laplace{f(t)e^{at}} = \bar{f}(s-a).
      \end{align*}
      As shown previously,
      \begin{align*}
        \bar{f}(s) = \laplace{f(t)} = \frac{n!}{s^{n+1}}.
      \end{align*}
      Therefore,
      \begin{align*}
        \laplace{t^n e^{at}} = \bar{f}(s-a) = \frac{n!}{(s-a)^{n+1}}.
      \end{align*}
  \end{enumerate}
\end{proof}
\newpage
