\begin{problem}{3.3}
  The following is a result relating the Laplace transform of a function's derivative
  to the Laplace transform of that function:
  \begin{align}\label{result}
    \laplace{f'(t)} = s \laplace{f(t)} - f(0).
  \end{align}
  Use the result to find
  \begin{enumerate}
    \item[a.] $\laplace{\cos at},$
    \item[b.] $\laplace{\sin at}$.
  \end{enumerate}
\end{problem}

\begin{proof}
  \begin{enumerate}
    \item[a.] Let $f(t) = \cos at$. Then $f'(t) = -a \sin at$ and from \eqref{result}
      we have
      \begin{align}\label{result_cos}
        -a \laplace{\sin at} = s \laplace{\cos at} - 1.
      \end{align}

      Now let $g(t) = \sin at$. Then $g'(t) = a \cos at$ and applying \eqref{result} to
      $g(t)$ yields
      \begin{align*}
        a \laplace{\cos at} = s \laplace{\sin at}.
      \end{align*}

      Therefore, from \eqref{result_cos} we have that
      \begin{align*}
        -a \left(\frac{a}{s} \laplace{\cos a t}\right) = s \laplace{\cos at} - 1
      \end{align*}
      which implies that
      \begin{align*}
        \laplace{\cos at} = \frac{s}{s^2 + a^2}.
      \end{align*}
    \item[b.]  Let $f(t) = \sin at$. Then $f'(t) = a \cos at$ and from \eqref{result}
      we have
      \begin{align}\label{result_sin}
        a \laplace{\cos at} = s \laplace{\sin at}.
      \end{align}

      Now let $g(t) = \cos at$. Then $g'(t) =- a \sin at$ and applying \eqref{result} to
      $g(t)$ yields
      \begin{align*}
        -a \laplace{\sin at} = s \laplace{\cos at} - 1
      \end{align*}
      which implies that
      \begin{align*}
        \laplace{\cos at} = \frac{1}{s} - \frac{a}{s} \laplace{\sin at}.
      \end{align*}

      Therefore, from \eqref{result_sin} we have that
      \begin{align*}
        a \left(\frac{1}{s} - \frac{a}{s}\laplace{\sin at}\right) = s \laplace{\sin at}
      \end{align*}
      which implies that
      \begin{align*}
        \laplace{\sin at} = \frac{a}{s^2 + a^2}.
      \end{align*}
  \end{enumerate}
\end{proof}
\newpage
