\begin{problem}{3.10}
  Show that
  \begin{enumerate}
    \item[a.] $\displaystyle \laplace{\frac{1}{t}(\sin at - at \cos at)} = \tan^{-1}\left(\frac{a}{s}\right) - \frac{as}{s^2 + a^2}$,
    \item[b.] $\displaystyle \laplace{\int_0^t \frac{1}{\tau}(\sin a \tau - a\tau \cos a\tau) d\tau} = \frac{1}{s}\left[\tan^{-1}\left(\frac{a}{s}\right) - \frac{as}{s^2 + a^2}\right]$.
  \end{enumerate}
\end{problem}

\begin{proof}
  \begin{enumerate}
    \item[a.] If $\bar{f}(s) = \laplace{f(t)}$, then from a previous theorem we have that
      \begin{align*}
        \laplace{\frac{f(t)}{t}} = \int_s^\infty \bar{f}(s) ds.
      \end{align*}
      Thus, we have that
      \begin{align*}
        \laplace{\frac{1}{t}(\sin at - at \cos at)}
        &= \int_s^\infty \laplace{\sin at - at \cos at}ds \\
        &= \int_s^\infty \laplace{\sin at} - a\laplace{t \cos at}ds.
      \end{align*}
      From our table of Laplace transforms,  we know that
      \begin{align*}
        \laplace{\sin at} = \frac{a}{s^2 + a^2}
      \end{align*}
      and
      \begin{align*}
        \laplace{t\cos at} = \frac{s^2 - a^2}{(s^2 + a^2)^2}.
      \end{align*}
      This implies that
      \begin{align*}
        \laplace{\frac{1}{t}(\sin at - at \cos at)}
        &= \int_s^\infty \laplace{\sin at} - a\laplace{t \cos at}ds \\
        &= \int_s^\infty \frac{a}{s^2 + a^2} - a\left(\frac{s^2 - a^2}{(s^2 + a^2)^2}\right)ds \\
        &= \left.\tan^{-1}\left(\frac{s}{a}\right)\right\rvert_s^\infty + \left.\frac{as}{s^2 + a^2}\right\rvert_s^\infty \\
        &= \frac{\pi}{2} - \tan^{-1}\left(\frac{s}{a}\right) - \frac{as}{s^2+a^2} \\
        &= \tan^{-1}\left(\frac{a}{s}\right) - \frac{as}{s^2 + a^2}.
      \end{align*}

    \item[b.] From the theorem regarding the Laplace transform of an integral, if $\bar{f}(s) = \laplace{f(t)}$,
      then
      \begin{align}\label{laplace_int}
        \laplace{\int_0^t f(\tau) d\tau} = \frac{\bar{f}(s)}{s}.
      \end{align}
      Suppose that $\displaystyle f(t) = \frac{1}{t}(\sin at - at \cos at)$. Then we have shown
      previously that
      \begin{align*}
        \bar{f}(s) = \laplace{f(t)} = \tan^{-1}\left(\frac{a}{s}\right) - \frac{as}{s^2 + a^2}.
      \end{align*}
      Therefore, we have by \eqref{laplace_int} that
      \begin{align*}
        \laplace{\int_0^t \frac{1}{\tau}(\sin a \tau - a\tau \cos a\tau) d\tau}
        &= \laplace{\int_0^t f(\tau) d\tau} \\
        &= \frac{\bar{f}(s)}{s} \\
        &= \frac{1}{s}\left[\tan^{-1}\left(\frac{a}{s}\right) - \frac{as}{s^2 + a^2}\right] .
      \end{align*}
  \end{enumerate}
\end{proof}
\newpage
