\begin{problem}{3.18}
  Establish the following result:
  \begin{enumerate}
    \item[a.] $\displaystyle \laplace{\sin^2 at} = \frac{2a^2}{s(s^2+4a^2)}.$
  \end{enumerate}
\end{problem}

\begin{proof}
  \begin{enumerate}
    \item[a.] Recall that $\cos 2\theta = 1 - 2\sin^2 \theta$. Thus,
      \begin{align*}
        \laplace{\sin^2 at} = \laplace{\frac{1}{2}\left(1 - \cos 2at \right)} = \frac{1}{2}\left[\laplace{1} - \laplace{\cos 2 at}\right].
      \end{align*}

      From our table of Laplace transforms, we know that
      \begin{align*}
        \laplace{1} = \frac{1}{s}
      \end{align*}
      and
      \begin{align*}
        \laplace{\cos b t} = \frac{s}{s^2 + b^2}
      \end{align*}
      which implies that
      \begin{align*}
        \laplace{\cos 2 at} = \frac{s}{s^2 + (2a)^2} = \frac{s}{s^2 + 4a^2}.
      \end{align*}
      Therefore, we have that
      \begin{align*}
        \laplace{\sin^2 at}
        &= \frac{1}{2}\left[\laplace{1} - \laplace{\cos 2 at}\right] \\
        &= \frac{1}{2}\left[\frac{1}{s} - \frac{s}{s^2+4a^2}\right] \\
        &= \frac{1}{2}\left[\frac{s^2 + 4a^2 - s^2}{s(s^2+4a^2)}\right] \\
        &= \frac{2a^2}{s(s^2 + 4a^2)}.
      \end{align*}
  \end{enumerate}
\end{proof}
\newpage
