\begin{problem}{3.7}
  Obtain the inverse Laplace transforms of the following functions:
  \begin{enumerate}
    \item[b.] $\displaystyle \bar{f}(s) = \frac{1}{s^2(s^2+c^2)}$.
  \end{enumerate}
\end{problem}

\begin{proof}
  \begin{enumerate}
    \item[b.] Let $\bar{f}(s) = \bar{g}(s)\bar{h}(s)$ where $\displaystyle \bar{g}(s) = \frac{1}{s^2}$
      and $\bar{h}(s) = \frac{1}{s^2+c^2}$.

      Using previous results, we know that
      \begin{align*}
        g(t) = \laplaceinv{\bar{g}(s)} = \laplaceinv{\frac{1}{s^2}} = t
      \end{align*}
      and
      \begin{align*}
        h(t) = \laplaceinv{\bar{h}(s)} = \laplaceinv{\frac{1}{c}\left(\frac{c}{s^2+c^2}\right)} = \frac{\sin ct}{c}.
      \end{align*}

      Now, by the Convolution Theorem for the Laplace transform, we have that
      \begin{align*}
        f(t) = \laplaceinv{\bar{f}(s)} = \laplaceinv{\bar{g}(s)\bar{h}(s)} = (g\ast h)(t)
      \end{align*}
      where
      \begin{align*}
        (g \ast h) (s) = \int_0^t g(t - \tau)h(\tau) d\tau.
      \end{align*}

      Therefore,
      \begin{align*}
        f(t) = (g \ast h)(t)
        &= \frac{1}{c}\int_0^t (t-\tau) \sin c \tau d\tau \\
        &= \frac{t}{c}\int_0^t \sin c\tau d\tau - \frac{1}{c} \int_0^t \tau \sin c\tau d\tau \\
        &= \frac{t}{c}\left[\frac{1}{c} - \frac{\cos ct}{c}\right] - \frac{1}{c}\left[-\frac{t\cos ct}{c} + \frac{\sin ct }{c^2}\right] \\
        &= \frac{t}{c^2} - \frac{\sin ct}{c^3}.
      \end{align*}
  \end{enumerate}
\end{proof}
\newpage
