\begin{problem}{1.1.3}
  A \emph{logistic difference equation} is one of the form $x_{n+1} = \mu x_{n} (1-x_n)$
  for some fixed $\mu \in \mathbb{R}$. Find exact (closed form) solutions to the following
  logistic difference equations:
  \begin{enumerate}
    \item $x_{n+1} = 2 x_{n} (1 - x_n)$. Hint: Use the substitution $x_n = (1 - y_n) / 2$
      to transform the equation into a simpler equation that is easily solved.
    \item $x_{n+1} = 4 x_n (1 - x_n)$. Hint: Set $x_n = \sin^2(\theta_n)$ and simplify
      to get an equation that is easily solved.
  \end{enumerate}
\end{problem}

\begin{proof}
  \begin{enumerate}
    \item Let $x_n = (1 - y_n) / 2$ for $n \in \mathbb{N}$ with $x_0$ given.
      Substituting this expression into the original difference equation yields the new
      difference equation
      \begin{align*}
        \frac{1 - y_{n+1}}{2} &= 2\left( \frac{1 - y_n}{2} \right) \left[ 1 - \left(\frac{1 - y_n}{2}\right) \right] \\
        &= (1 - y_n)\left(\frac{1 + y_n}{2}\right) \\
        &= \frac{1 - y_n^2}{2}.
      \end{align*}
      This new difference equation reduces to $y_{n+1} = y_n^2$ for $n\in\mathbb{N}$,
      the solution of which is readily seen to be $y_{n+1} = y_0 ^{2^{n+1}}$. Making
      the substitution $y_n = 1 - 2 x_n$ shows that, for $n\in\mathbb{N}$,
      the solution to the original difference equation is given by
      \begin{align*}
        x_{n+1} = \frac{1 - (1- 2x_0)^{2^{n+1}}}{2}.
      \end{align*}
    \item Let $x_n = \sin^2(\theta_n)$ for $n \in \mathbb{N}$ with $x_0$ given.
      We may assume without loss of generality that $\theta_n \in [0, \pi)$ for
      if the angle $\theta_n$ isn't in the stated range, we can find an integer $k$ such that
      $\theta_n + k \pi \in [0, \pi)$ and $\sin^2(\theta_n) = \sin^2(\theta_n + k\pi)$. We then declare the sum $\theta_n + k \pi$ to be the new angle $\theta_n$.
      Substituting the above expression for $x_n$ into the original difference equation yields the new
      difference equation
      \begin{align*}
        \sin^2(\theta_{n+1}) &= 4 \sin^2(\theta_{n}) \left( 1 - \sin^2(\theta_{n})\right)\\
        &= \left(2 \sin(\theta_n) \cos(\theta_n)\right)^2 \\
        &= \sin^2(2\theta_n).
      \end{align*}
      Knowing that for $x, y \in [0, \pi)$ we have that $\sin^2(x) = \sin^2(y)$ if and only if $x = y$,
      the new difference equation reduces to $\theta_{n+1} = 2\theta_n$ for $n\in\mathbb{N}$ where it is implicitly
      understood that $\theta_{n+1}$ will be mapped to the corresponding angle between 0 and $\pi$ if
      $2\theta_n \geq \pi$.
      Using the closed form solution for difference equations in the form of linear maps,
      the solution to the reduced difference equation is given by $\theta_{n+1} = 2^{n+1}\theta_0$
      for $n\in\mathbb{N}$. Making the substitution $\theta_n =  \sin^{-1}(\sqrt{x_n})$ shows that, for $n\in\mathbb{N}$,
      the solution to the original difference equation is given by
      \begin{align*}
        x_{n+1} = \sin^2(2^{n+1}\sin^{-1}(\sqrt{x_0})).
      \end{align*}

  \end{enumerate}
\end{proof}
\newpage
