\begin{problem}{2.8.3}
  Show that
  \begin{align*}
    \left\{\frac{\mu}{1+\mu^3}, \frac{\mu^2}{1+\mu^3}, \frac{\mu^3}{1+\mu^3}\right\}
  \end{align*}
  is a 3-cycle for $T_\mu$ when $\mu \geq (1+\sqrt{5})/2$.
\end{problem}

\begin{proof}
  The tent map is defined as
  \begin{align*}
    T_\mu(x) :=
    \begin{cases}
      \mu x & 0 \leq x \leq 1/2 \\
      \mu (1- x) & 1/2 < x \leq 1
    \end{cases}.
  \end{align*}

  Now suppose that $\mu \geq (1+\sqrt{5})/2 > 1$ and let $x_1 = \frac{\mu}{1+\mu^3}$.
  We will now show that
  \begin{align*}
    T_\mu(x_1) = \frac{\mu^2}{1+\mu^3} = x_2, \quad T_\mu^2(x_1) = T_\mu(x_2) = \frac{\mu^3}{1+\mu^3} = x_3, \quad T_\mu^3(x_1) = T_\mu(x_3) = \frac{\mu}{1+\mu^3} = x_1
  \end{align*}
  demonstrating that $\{x_1, x_2, x_3\}$ is a 3-cycle.

  Note that $\mu / (1+\mu^3)$ is monotonically decreasing if $\mu \geq (1 + \sqrt{5})/2$. Thus,
  \begin{align*}
    0 \leq \frac{\mu}{1+\mu^3} \leq \frac{\frac{1 + \sqrt{5}}{2}}{1 + \left(\frac{1 + \sqrt{5}}{2}\right)^3} = \frac{-1 + \sqrt{5}}{4} \leq \frac{1}{2}.
  \end{align*}
  Hence,
  \begin{align*}
    T_\mu(x_1) = \mu\left(\frac{\mu}{1 + \mu^3}\right) = \frac{\mu^2}{1 + \mu^3} = x_2.
  \end{align*}
  Similarly, we see that $\mu^2 / (1+\mu^3)$ is monotonically decreasing if $\mu\geq (1 + \sqrt{5})/2$ so
  \begin{align*}
    0 \leq \frac{\mu^2}{1+\mu^3} \leq \frac{\left(\frac{1 + \sqrt{5}}{2}\right)^2}{1 + \left(\frac{1 + \sqrt{5}}{2}\right)^3} = \frac{1}{2}.
  \end{align*}
  Thus,
  \begin{align*}
    T_\mu(x_2) = \mu\left(\frac{\mu^2}{1 + \mu^3}\right) = \frac{\mu^3}{1 + \mu^3} = x_3.
  \end{align*}
  Lastly, if $\mu \geq (1 + \sqrt{5})/2$ then $\mu^3 / (1+\mu^3)$ is monotonically
  increasing so that
  \begin{align*}
    \frac{1}{2} \leq \frac{1 + \sqrt{5}}{4} = \frac{\left(\frac{1 + \sqrt{5}}{2}\right)^3}{1 + \left(\frac{1 + \sqrt{5}}{2}\right)^3} \leq \frac{\mu^3}{1+\mu^3} \leq 1
  \end{align*}

  Therefore,
  \begin{align*}
    T_\mu(x_3)
    &= \mu\left(1-\frac{\mu^3}{1 + \mu^3}\right) = \frac{\mu }{1 + \mu^3} = x_1
  \end{align*}
  and $\{x_1, x_2, x_3\}$ is a 3-cycle.

\end{proof}
\newpage
