\begin{problem}{12.1}
  Find the $Z$-transform of the following functions:
  \begin{enumerate}
    \item[a.] $f(n) = n^3$,
    \item[b.] $\displaystyle f(n) = \frac{a^n}{n!}$
  \end{enumerate}
\end{problem}

\begin{proof}
  For a function $f(n)$, the $Z$-transform of $f(n)$ is defined as
  \begin{align*}
    \Z{f(n)} = F(z) = \sum_{n=0}^\infty f(n) z^{-n}.
  \end{align*}
  \begin{enumerate}
    \item[a.] Let $g(n) = n^2$ and $f(n) = n^3 = n g(n)$.
      From our table of $Z$-transforms we know that
      \begin{align*}
        G(z) = \Z{g(n)} = \sum_{n=0}^{\infty} n^2 z^{-n} = \frac{z(z+1)}{(z-1)^3}
      \end{align*}
      given that $|z| > 1$.
      The multiplication theorem states that if $F(z) = \Z{f(n)}$, then
      \begin{align*}
        \Z{n f(n)} = -z \der{z}{}\left[F(z)\right].
      \end{align*}
      Thus, we have that
      \begin{align*}
        F(z) = \Z{f(n)} &= \Z{n g(n)} \\
        &= -z \der{z}{}\left[\frac{z(z+1)}{(z-1)^3}\right] \\
        &= \frac{z(z^2 + 4z + 1)}{(z-1)^4}
      \end{align*}

    \item[b.] Let $g(n) = \frac{1}{n!}$ and $f(n) = \frac{a^n}{n!} = a^n g(n)$.
      From our knowledge of infinite series, we know from the definition of the $Z$-transform that
      \begin{align*}
        G(z) = \Z{g(n)} &= \sum_{n=0}^\infty \frac{z^{-n}}{n!} = e^{\frac{1}{z}}.
      \end{align*}
      From the multiplication theorem, if $F(z) = \Z{f(n)}$, then
      \begin{align*}
        \Z{a^n f(n)} = F\left(\frac{z}{a}\right).
      \end{align*}
      Therefore, we have that
      \begin{align*}
        F(z) = \Z{f(n)} = \Z{a^ng(n)} &= G\left(\frac{z}{a}\right) = e^{\frac{a}{z}}.
      \end{align*}
  \end{enumerate}
\end{proof}
\newpage
