\begin{problem}{12.3}
  Show that
  \begin{align*}
    \Z{n a^n f(n)} = -z \der{z}{}\left[F\left(\frac{z}{a}\right)\right].
  \end{align*}
\end{problem}

\begin{proof}
  Suppose that $G(z) = \Z{g(n)}$. Then the multiplication theorem states that
  \begin{align}
    \label{mult:1}
    \Z{a^n g(n)} = G\left(\frac{z}{a}\right)
  \end{align}
  and
  \begin{align}
    \label{mult:2}
    \Z{n g(n)} = -z \der{z}{}\left[G(z)\right].
  \end{align}

  Let $g(n) = a^n f(n)$ and suppose that $F(z) = \Z{f(n)}$. By \eqref{mult:1}, we have that
  \begin{align*}
    G(z) = \Z{g(n)} = \Z{a^n f(n)} = F\left(\frac{z}{a}\right).
  \end{align*}
  Therefore, by \eqref{mult:2}, we have that
  \begin{align*}
    \Z{n a^n f(n)} = \Z{n g(n)} = -z \der{z}{}\left[G(z)\right] = -z \der{z}{}\left[F\left(\frac{z}{a}\right)\right].
  \end{align*}
\end{proof}
\newpage
