\begin{problem}{12.5}
  Show that
  \begin{enumerate}
    \item[a.] $\displaystyle \Z{n a^{n-1}} = \sum_{n=0}^\infty \frac{z}{(z-a)^2}.$
  \end{enumerate}
\end{problem}

\begin{proof}
  \begin{enumerate}
    \item[a.] Let $f(n) = a^{n-1}$. Then from the definition of the $Z$-transform,
      we have that
      \begin{align*}
        F(z) = \Z{f(n)} &= \sum_{n=0}^\infty a^{n-1} z^{-n} \\
        &= \frac{1}{a}\sum_{n=0}^\infty \left(\frac{z}{a}\right)^{-n} \\
        &= \frac{z}{a(z-a)}.
      \end{align*}

      By the multiplication theorem \eqref{mult:2}, we
      therefore have that
      \begin{align*}
        \Z{n a^{n-1}} = \Z{n f(n)} &= -z \der{z}{}\left[F(z)\right]\\
        &= -z \frac{a(z-a) - za}{a^2(z-a)^2} \\
        &= \frac{z}{(z-a)^2}.
      \end{align*}
  \end{enumerate}
\end{proof}
\newpage
